simplied the invariant for promotable allocas. It does not require promotable allocas are dominators, but only defined. When the invariant is used, we must know the allocas are in scope, and are defined.
git-svn-id: https://webdav.seas.upenn.edu/svn/sol/vol@3583 eef5ea85-cc2e-0410-bd84-0fae1f012da8

src/Transforms/promotable_props.v
@@ -64,21 +64,14 @@ exists gv,
   mload TD Mem gvsa (PI_typ pinfo) (PI_align pinfo) = Some gv.
 
 Definition wf_defs (maxb:Values.block) (pinfo:PhiInfo) TD M (lc:DGVMap) 
-  (ids0:list atom) (als:list Values.block) : Prop :=
+  (als:list Values.block) : Prop :=
 forall gvsa
-  (Hinp: In (PI_id pinfo) ids0)
   (Hlkp: lookupAL _ lc (PI_id pinfo) = Some gvsa),
   wf_alloca_GVs maxb pinfo TD M gvsa als /\
   (forall id0 gvs0 
    (*Hin0: In id0 ids0*) 
    (Hlk0: lookupAL _ lc id0 = Some gvs0),
    wf_non_alloca_GVs pinfo id0 gvs0 gvsa).
-
-Definition inscope_of_pc f b cs tmn : option (list id) :=
-match cs with
-| nil => inscope_of_tmn f b tmn
-| c::_ => inscope_of_cmd f b c
-end.
 
 (* Except domination property, the other properties are the same for a lot of 
    proofs, we should prove them all for once. Or, we do not need to use them
@@ -87,21 +80,14 @@ end.
 Definition wf_ExecutionContext (maxb:Values.block) (pinfo:PhiInfo) TD M 
   (ec:Opsem.ExecutionContext) : Prop :=
 let '(Opsem.mkEC f b cs tmn lc als) := ec in
-(if (fdef_dec (PI_f pinfo) f) then 
-  match inscope_of_pc f b cs tmn with
-  | Some ids => wf_defs maxb pinfo TD M lc ids als
-  | None => False
-  end
-else True)
+(if (fdef_dec (PI_f pinfo) f) then wf_defs maxb pinfo TD M lc als else True)
 /\ wf_lc M lc.
 
 Definition wf_ECStack_head_in_tail (maxb:Values.block) (pinfo:PhiInfo) TD M 
   (lc:DGVMap) (ec0:Opsem.ExecutionContext) : Prop :=
 let '(Opsem.mkEC f0 b0 cs0 tmn0 lc0 _) := ec0 in
-forall ids0 gvsa, 
+forall gvsa, 
   f0 = PI_f pinfo ->
-  inscope_of_pc f0 b0 cs0 tmn0 = Some ids0 -> 
-  In (PI_id pinfo) ids0 ->
   lookupAL _ lc0 (PI_id pinfo) = Some gvsa ->
   (exists mb, gvsa = ($ (blk2GV TD mb) # (typ_pointer (PI_typ pinfo)) $) /\ 
     maxb < mb < Mem.nextblock M) /\
@@ -135,20 +121,10 @@ wf_als maxb M
   (flat_map (fun ec => let '(Opsem.mkEC _ _ _ _ _ als) := ec in als) ecs) /\
 wf_Mem maxb td M.
 
-Lemma wf_defs_eq : forall maxb pinfo TD M lc ids1 ids2 als,
-  AtomSet.set_eq _ ids1 ids2 ->
-  wf_defs maxb pinfo TD M lc ids1 als ->
-  wf_defs maxb pinfo TD M lc ids2 als.
-Proof.
-  intros. unfold wf_defs in *. intros.
-  destruct H as [H1 H2]. eauto.
-Qed.
-
 Definition wf_GVs (maxb:Values.block)(pinfo:PhiInfo)(TD:targetdata)(M:mem)
-  (lc:DGVMap)(ids1:list id)(als:list Values.block)(id1:id)(gv1:GVsT DGVs)
+  (lc:DGVMap)(als:list Values.block)(id1:id)(gv1:GVsT DGVs)
   : Prop :=
   (forall gvsa,
-     In (PI_id pinfo) ids1 ->
      lookupAL _ lc (PI_id pinfo) = Some gvsa ->
      no_alias gv1 gvsa) /\
   (id1 = (PI_id pinfo) ->
@@ -157,16 +133,13 @@ Definition wf_GVs (maxb:Values.block)(pinfo:PhiInfo)(TD:targetdata)(M:mem)
         no_alias gvs0 gv1) /\
      wf_alloca_GVs maxb pinfo TD M gv1 als).
 
-Lemma wf_defs_updateAddAL: forall maxb pinfo TD M lc' ids1 ids2 i1 gv1 als
-  (HwfDef: wf_defs maxb pinfo TD M lc' ids1 als)
-  (Heq: AtomSet.set_eq _ (i1::ids1) ids2)
-  (Hwfgvs: wf_GVs maxb pinfo TD M lc' ids1 als i1 gv1),
-  wf_defs maxb pinfo TD M (updateAddAL _ lc' i1 gv1) ids2 als.
+Lemma wf_defs_updateAddAL: forall maxb pinfo TD M lc' i1 gv1 als
+  (HwfDef: wf_defs maxb pinfo TD M lc' als)
+  (Hwfgvs: wf_GVs maxb pinfo TD M lc' als i1 gv1),
+  wf_defs maxb pinfo TD M (updateAddAL _ lc' i1 gv1) als.
 Proof.
   intros. unfold wf_defs. intros.
   destruct Hwfgvs as [Hwfgvs1 Hwfgvs2].
-  destruct Heq as [Hinc1 Hinc2].
-  apply Hinc2 in Hinp. simpl in Hinp.
   destruct (eq_dec i1 (PI_id pinfo)); subst.
     rewrite lookupAL_updateAddAL_eq in Hlkp.
     inv Hlkp.
@@ -179,7 +152,6 @@ Proof.
 
     clear Hwfgvs2.
     rewrite <- lookupAL_updateAddAL_neq in Hlkp; auto.
-    destruct Hinp as [EQ | Hinp]; subst; try congruence.
     assert (Hlkp':=Hlkp).
     apply HwfDef in Hlkp; auto.
     destruct Hlkp as [J1 J2].
@@ -238,11 +210,9 @@ Lemma impure_cmd_non_updated_preserves_wf_EC : forall maxb pinfo TD M M' lc F B
   (HFinPs: InProductsB (product_fdef F) Ps = true)
   (HBinF: blockInFdefB B F = true)
   (Hid : getCmdID c0 = None)
-  (Hwfdefs: forall ids0,
-              F = (PI_f pinfo) ->
-              inscope_of_pc F B (c0::cs) tmn = Some ids0 ->
-              wf_defs maxb pinfo TD M lc ids0 als ->
-              wf_defs maxb pinfo TD M' lc ids0 als)
+  (Hwfdefs:   F = (PI_f pinfo) ->
+              wf_defs maxb pinfo TD M lc als ->
+              wf_defs maxb pinfo TD M' lc als)
   (Hwflc: wf_lc M lc -> wf_lc M' lc)
   (HwfEC: wf_ExecutionContext maxb pinfo TD M 
             {| Opsem.CurFunction := F;
@@ -263,48 +233,6 @@ Proof.
   destruct HwfEC as [J1 J2].
   split; auto.
   destruct (fdef_dec (PI_f pinfo) F); subst; auto.
-  remember (inscope_of_cmd (PI_f pinfo) 
-    (block_intro l1 ps1 (cs1' ++ c0 :: cs) tmn) c0) as R1. 
-  assert (HeqR1':=HeqR1).
-  unfold inscope_of_cmd, inscope_of_id in HeqR1'.
-
-  destruct R1; try solve [inversion J1].
-  repeat (split; try solve [auto]).
-      unfold inscope_of_pc.
-      destruct cs; simpl_env in *.
-      SSSSCase "cs = nil".
-        assert (~ In (getCmdLoc c0) (getCmdsLocs cs1')) 
-          as Hnotin.
-          eapply preservation_helper1; eauto.
-
-        apply inscope_of_cmd_tmn in HeqR1; auto.
-        destruct HeqR1 as [ids2 [J1' J2']].
-        rewrite <- J1'.
-        assert (In c0 (cs1' ++ [c0])) as HinCs.
-          apply in_or_app. right. simpl. auto.
-        assert (Hwfc := HBinF).
-        eapply wf_system__wf_cmd with (c:=c0) in Hwfc; 
-          eauto.
-        assert (HwfF:=HFinPs). eapply wf_system__wf_fdef in HwfF; eauto.
-        rewrite Hid in J2'. 
-        eapply wf_defs_eq; eauto.       
-
-      SSSSCase "cs <> nil".
-        assert (NoDup (getCmdsLocs (cs1' ++ [c0] ++ [c] ++ cs))) 
-          as Hnodup.
-          eapply preservation_helper2; eauto.
-
-        apply inscope_of_cmd_cmd in HeqR1; auto.
-        destruct HeqR1 as [ids2 [J1' J2']].        
-        rewrite <- J1'.
-        assert (In c0 (cs1' ++ [c0] ++ [c] ++ cs)) 
-          as HinCs.
-          apply in_or_app. right. simpl. auto.
-        assert (Hwfc := HBinF).
-        eapply wf_system__wf_cmd with (c:=c0) in Hwfc; 
-          eauto.
-        rewrite Hid in J2'. 
-        eapply wf_defs_eq; eauto.
 Qed.
 
 (* We need a generic proof for this one and the one for atom *)
@@ -418,23 +346,17 @@ Proof.
   eapply cgv2gvs_preserves_valid_ptrs; eauto; try omega.
 Qed.
 
-Definition inscope_of_EC (ec:@Opsem.ExecutionContext DGVs) : option (list id) :=
-let '(Opsem.mkEC f b cs tmn _ _) := ec in inscope_of_pc f b cs tmn.
-
 Lemma preservation_return_helper: forall (g : GVsT DGVs) pinfo lc' Mem'
   als' td maxb Mem ECs lc gl t Result
   (HeqR1 : ret g = Opsem.getOperandValue td Result lc gl)
   (g0 : GVsT DGVs)
   (HeqR2 : ret g0 = lift_op1 DGVs (fit_gv td t) g t)
-  (Hwfg : wf_globals maxb gl)
-  (l0 : list atom) EC
+  (Hwfg : wf_globals maxb gl) EC
   (Heq1 : Opsem.CurFunction EC = PI_f pinfo)
   (Heq2 : Opsem.Locals EC = lc')
   (Hfr1 : wf_ECStack_head_tail maxb pinfo td Mem lc (EC :: ECs))
-  (Hinscp: inscope_of_EC EC = Some l0)
-  (Hinscope2 : wf_defs maxb pinfo td Mem' lc' l0 als')
+  (Hinscope2 : wf_defs maxb pinfo td Mem' lc' als')
   (gvsa : GVsT DGVs)
-  (Hpindom : In (PI_id pinfo) l0)
   (Hlkp : lookupAL (GVsT DGVs) lc' (PI_id pinfo) = ret gvsa),
   no_alias g0 gvsa.
 Proof.
@@ -457,6 +379,7 @@ Proof.
       omega.
   
     eapply undef_disjoint_with_ptr; eauto.
+  Opaque lift_op1.
 Qed.
 
 Ltac SSSSSCase name := Case_aux subsubsubsubsubcase name.
@@ -470,8 +393,8 @@ Proof.
   unfold wf_ECStack_head_tail, wf_ECStack_head_in_tail.
   intros. destruct ec0. intros.
   eapply Hwf in H; eauto. clear Hwf.
-  eapply H in H2; eauto. clear H.
-  destruct H2 as [[mb [J11 J12]] [J2 J3]]; subst.
+  eapply_clear H in H1.
+  destruct H1 as [[mb [J11 J12]] [J2 J3]]; subst.
   split.
     exists mb. split; auto. 
     erewrite <- nextblock_free; eauto.
@@ -485,9 +408,7 @@ Lemma operand__no_alias_with__tail: forall maxb pinfo TD M lc1 lc2 mptr0 gl
   (Heq1: Opsem.CurFunction EC = PI_f pinfo)
   (Heq2: Opsem.Locals EC = lc2)
   (Hht : wf_ECStack_head_in_tail maxb pinfo TD M lc1 EC)
-  (gvsa : GVsT DGVs) (Hin: mptr0 @ mptrs) ids0
-  (Heq3 : inscope_of_EC EC = Some ids0)
-  (Hin: In (PI_id pinfo) ids0)
+  (gvsa : GVsT DGVs) (Hin: mptr0 @ mptrs)
   (Hlkp : lookupAL (GVsT DGVs) lc2 (PI_id pinfo) = ret gvsa)
   (Hgetop : Opsem.getOperandValue TD v lc1 gl = ret mptrs),
   no_alias mptr0 gvsa.
@@ -502,12 +423,8 @@ Proof.
       omega.
 Qed.
 
-Definition wf_use_at_head (pinfo:PhiInfo) (ids0:list id) (v:value) :=
-used_in_value (PI_id pinfo) v = false /\
-match v with
-| value_const _ => True
-| value_id vid => In vid ids0
-end.
+Definition wf_use_at_head (pinfo:PhiInfo) (v:value) :=
+used_in_value (PI_id pinfo) v = false.
 
 Lemma free_preserves_wf_defs_in_tail : forall maxb pinfo TD M  
   M' lc1 mptr0 mptrs gl v als lc2 
@@ -517,12 +434,11 @@ Lemma free_preserves_wf_defs_in_tail : forall maxb pinfo TD M
   (Heq1: Opsem.CurFunction EC = PI_f pinfo)
   (Heq2: Opsem.Locals EC = lc2)
   (Hht: wf_ECStack_head_in_tail maxb pinfo TD M lc1 EC)
-  ids0 (Heq3 : inscope_of_EC EC = Some ids0)
-  (Hwf: wf_defs maxb pinfo TD M lc2 ids0 als),
-  wf_defs maxb pinfo TD M' lc2 ids0 als.
+  (Hwf: wf_defs maxb pinfo TD M lc2 als),
+  wf_defs maxb pinfo TD M' lc2 als.
 Proof.
   intros. unfold wf_defs. 
-  intros gvsa Hpindom Hlkp.
+  intros gvsa Hlkp.
   assert (Hlkp':=Hlkp).
   apply Hwf in Hlkp'; auto.
   destruct Hlkp' as [J1 J2].
@@ -542,10 +458,9 @@ Qed.
 
 Lemma operand__no_alias_with__head: forall maxb pinfo TD lc mptr0 mptrs gl v als
   (Hgetop : Opsem.getOperandValue TD v lc gl = ret mptrs)
-  (Hin : mptr0 @ mptrs) (Hwfgl : wf_globals maxb gl) ids0 M
-  (Hwfu: wf_use_at_head pinfo ids0 v) (Hwf: wf_defs maxb pinfo TD M lc ids0 als)
-  (gvsa : GVsT DGVs) (Hpindom : In (PI_id pinfo) ids0)
-  (Hlkp : lookupAL (GVsT DGVs) lc (PI_id pinfo) = ret gvsa),
+  (Hin : mptr0 @ mptrs) (Hwfgl : wf_globals maxb gl) M
+  (Hwfu: wf_use_at_head pinfo v) (Hwf: wf_defs maxb pinfo TD M lc als)
+  (gvsa : GVsT DGVs) (Hlkp : lookupAL (GVsT DGVs) lc (PI_id pinfo) = ret gvsa),
   no_alias mptr0 gvsa.
 Proof.
   intros.
@@ -553,11 +468,10 @@ Proof.
   destruct Hlkp as [[J1 [J4 [gv J3]]] J2].
   inv Hin.
   destruct v; simpl in Hgetop.
-    destruct Hwfu as [Hwfu1 Hwfu2].        
     apply J2 in Hgetop; auto.
     unfold wf_non_alloca_GVs in Hgetop.
     destruct (id_dec i0 (PI_id pinfo)); subst; auto.
-      inv Hwfu1. 
+      inv Hwfu. 
       destruct (id_dec (PI_id pinfo) (PI_id pinfo)); try congruence.
         inv H0.
   
@@ -571,12 +485,12 @@ Lemma free_preserves_wf_defs_at_head : forall maxb pinfo TD M
   (Hgetop: Opsem.getOperandValue TD v lc gl = ret mptrs)
   (Hin: mptr0 @ mptrs) (Hwfgl: wf_globals maxb gl)
   (Hfree: free TD M mptr0 = ret M')
-  ids0 (Hwfu: wf_use_at_head pinfo ids0 v) 
-  (Hwf: wf_defs maxb pinfo TD M lc ids0 als),
-  wf_defs maxb pinfo TD M' lc ids0 als.
+  (Hwfu: wf_use_at_head pinfo v) 
+  (Hwf: wf_defs maxb pinfo TD M lc als),
+  wf_defs maxb pinfo TD M' lc als.
 Proof.
   intros. unfold wf_defs. 
-  intros gvsa Hpindom Hlkp.
+  intros gvsa Hlkp.
   assert (no_alias mptr0 gvsa) as J.
     eapply operand__no_alias_with__head; eauto.
   assert (Hlkp':=Hlkp).
@@ -604,12 +518,11 @@ Qed.
 
 Lemma impure_cmd_preserves_wf_EC_tail : forall maxb pinfo TD M  
   M' EC (Hwfpi: WF_PhiInfo pinfo) 
-  (Hwfdefs: forall ids0,
+  (Hwfdefs:
      let '(Opsem.mkEC F B cs tmn lc als) := EC in
      F = (PI_f pinfo) ->
-     inscope_of_pc F B cs tmn = Some ids0 ->
-     wf_defs maxb pinfo TD M lc ids0 als ->
-     wf_defs maxb pinfo TD M' lc ids0 als)
+     wf_defs maxb pinfo TD M lc als ->
+     wf_defs maxb pinfo TD M' lc als)
   (Hwflc: wf_lc M (@Opsem.Locals DGVs EC) -> wf_lc M' (Opsem.Locals EC))
   (Hwf: wf_ExecutionContext maxb pinfo TD M EC),
   wf_ExecutionContext maxb pinfo TD M' EC.
@@ -618,13 +531,6 @@ Proof.
   destruct Hwf as [J1 J2].
   split; auto.
     destruct (fdef_dec (PI_f pinfo) CurFunction); subst; auto.
-    unfold inscope_of_pc in *.
-    destruct CurCmds.    
-      remember (inscope_of_tmn (PI_f pinfo) CurBB Terminator) as R.
-      destruct R; auto.
-
-      remember (inscope_of_cmd (PI_f pinfo) CurBB c) as R.
-      destruct R; auto.
 Qed.
 
 Lemma free_preserves_wf_ECStack_in_tail : forall maxb pinfo TD M  
@@ -689,11 +595,11 @@ Proof.
     eapply NoDup_disjoint in H0; eauto.
 Qed.
 
-Lemma free_allocas_preserves_wf_defs: forall maxb pinfo TD Mem lc' l0 als0 als Mem',
-  wf_defs maxb pinfo TD Mem lc' l0 als0 ->
+Lemma free_allocas_preserves_wf_defs: forall maxb pinfo TD Mem lc' als0 als Mem',
+  wf_defs maxb pinfo TD Mem lc' als0 ->
   NoDup (als ++ als0) ->
   free_allocas TD Mem als = ret Mem' ->
-  wf_defs maxb pinfo TD Mem' lc' l0 als0.
+  wf_defs maxb pinfo TD Mem' lc' als0.
   (* This is only true if als is always disjoint with pinfo.id *) 
 Proof.
   intros. unfold wf_defs in *. intros.
@@ -737,6 +643,7 @@ Proof.
     inv_mbind. 
     apply updateAddAL__wf_lc; auto.
     intros. subst. symmetry in HeqR.
+Local Transparent lift_op1. unfold lift_op1 in HeqR0. simpl in HeqR0.
     unfold MDGVs.lift_op1, fit_gv in HeqR0. symmetry in HeqR0.
     inv_mbind. 
     destruct (sizeGenericValue g =n= nat_of_Z (ZRdiv (Z_of_nat n) 8)).
@@ -744,6 +651,7 @@ Proof.
       eapply operand__lt_nextblock in HeqR; eauto.
 
       unfold gundef in H0. inv_mbind. simpl. auto.
+Opaque lift_op1.
 Qed.
 
 Lemma free_allocas_preserves_wf_ECStack_head_tail' : forall maxb pinfo td 
@@ -761,9 +669,9 @@ Proof.
 Qed.
 
 Lemma free_allocas_preserves_wf_defs_in_tail : forall maxb pinfo TD
-  lc2 ids0 als' als M M' (Hfree: free_allocas TD M als = ret M')
-  (Hndp: NoDup (als++als')) (Hwf: wf_defs maxb pinfo TD M lc2 ids0 als'),
-  wf_defs maxb pinfo TD M' lc2 ids0 als'.
+  lc2 als' als M M' (Hfree: free_allocas TD M als = ret M')
+  (Hndp: NoDup (als++als')) (Hwf: wf_defs maxb pinfo TD M lc2 als'),
+  wf_defs maxb pinfo TD M' lc2 als'.
 Proof.
   induction als; simpl; intros.
     inv Hfree. auto.
@@ -772,7 +680,7 @@ Proof.
     apply IHals in H0; auto.
 
   unfold wf_defs. 
-  intros gvsa Hpindom Hlkp.
+  intros gvsa Hlkp.
   assert (Hlkp':=Hlkp).
   apply Hwf in Hlkp'; auto.
   destruct Hlkp' as [J1 J2].
@@ -832,8 +740,7 @@ Qed.
 
 Lemma updateAddAL__wf_ECStack_head_tail: forall maxb pinfo td M lc ECs
   id0 gv3 
-  (Hwfgv: forall ec0 (Hin : In ec0 ECs) (gvsa : GVsT DGVs) ids0
-    (Hscp: inscope_of_EC ec0 = Some ids0) (Hin1: In (PI_id pinfo) ids0)
+  (Hwfgv: forall ec0 (Hin : In ec0 ECs) (gvsa : GVsT DGVs)
     (Heq : Opsem.CurFunction ec0 = PI_f pinfo)
     (Hlkup : lookupAL (GVsT DGVs) (Opsem.Locals ec0) (PI_id pinfo) = ret gvsa),
     no_alias gv3 gvsa),
@@ -844,8 +751,8 @@ Proof.
   intros. destruct ec0. intros.
   assert (H0':=H0). eapply Hwfgv in H0'; eauto. clear Hwfgv.
   apply H in H0; auto. clear H. 
-  eapply H0 in H4; eauto. clear H0.
-  destruct H4 as [J1 [J2 J3]].
+  eapply_clear H0 in H2.
+  destruct H2 as [J1 [J2 J3]].
   split; auto.
   split; auto.
     intros. 
@@ -855,6 +762,8 @@ Proof.
 
       rewrite <- lookupAL_updateAddAL_neq in H; eauto.
 Qed.
+
+Local Transparent lift_op1. 
 
 Lemma free_allocas_preserves_wf_ECStack_head_tail : forall maxb pinfo td M M' 
   lc als lc' F' lc'' ECs gl Result c' EC
@@ -898,6 +807,401 @@ Proof.
 Local Transparent gv2gvs.
       unfold gv2gvs. simpl. auto.
 Opaque gv2gvs. 
+Qed.
+
+Lemma NoDup_split': forall A (l1 l2:list A),
+  NoDup (l1++l2) ->
+  NoDup l1 /\ NoDup l2 /\ (forall (a:A), In a l1 -> ~ In a l2).
+Proof.
+  induction l1; simpl; intros; auto.
+    inv H.
+    apply IHl1 in H3. destruct H3 as [J1 [J2 J3]].
+    split.
+      constructor; auto.
+        intro J. apply H2. apply in_or_app; auto.
+    split; auto.
+      intros. 
+      destruct H as [H | H]; subst; auto.
+        intro J. apply H2. apply in_or_app; auto.
+Qed.
+
+Lemma IngetCmdsLocs__lookupCmdViaIDFromCmds: forall c1 cs1
+  (Huniq: NoDup (getCmdsLocs cs1)) (H0 : In c1 cs1),
+  lookupCmdViaIDFromCmds cs1 (getCmdLoc c1) = Some c1.
+Proof.
+  induction cs1; simpl; intros.
+    inv H0.
+
+    destruct H0 as [H0 | H0]; subst.
+      destruct (eq_atom_dec (getCmdLoc c1) (getCmdLoc c1)); auto.
+        congruence.
+      inv Huniq.
+      destruct (eq_atom_dec (getCmdLoc c1) (getCmdLoc a)); auto.
+        contradict H2. rewrite <- e. apply In_InCmdLocs; auto. 
+Qed.
+
+Lemma IngetCmdsIDs__lookupCmdViaIDFromFdef: forall c1 l1 ps1 cs1 tmn1 f
+  (Huniq: uniqFdef f)
+  (H : blockInFdefB (block_intro l1 ps1 cs1 tmn1) f = true)
+  (H0 : In c1 cs1),
+  lookupInsnViaIDFromFdef f (getCmdLoc c1) = Some (insn_cmd c1).
+Proof.
+  destruct f as [[] bs]. simpl. intros.
+  destruct Huniq as [_ Huniq].
+  apply NoDup_split in Huniq.
+  destruct Huniq as [_ Huniq].
+  generalize dependent l1.
+  generalize dependent ps1.
+  generalize dependent cs1.
+  generalize dependent tmn1.
+  induction bs; simpl; intros.
+    inv H.
+
+    simpl in Huniq.
+    apply NoDup_split' in Huniq.
+    destruct Huniq as [J1 [J2 J3]].
+    apply orb_true_iff in H.
+    destruct H as [H | H].
+      apply blockEqB_inv in H.
+      subst. simpl.
+      assert (~ In (getCmdLoc c1) (getPhiNodesIDs ps1)) as Hnotin.
+        simpl in J1. 
+        apply infrastructure_props.NoDup_disjoint with (i0:=getCmdLoc c1) 
+          in J1; auto.
+        apply in_or_app. left. apply In_InCmdLocs; auto.
+      rewrite notin__lookupPhiNodeViaIDFromPhiNodes_none; auto.
+      simpl in J1. apply NoDup_inv in J1. destruct J1 as [_ J1].
+      apply NoDup_inv in J1. destruct J1 as [Huniq _].
+      rewrite IngetCmdsLocs__lookupCmdViaIDFromCmds; auto.
+
+      assert (~ In (getCmdLoc c1) (getBlockLocs a0)) as Hnotin.     
+        intro J. apply J3 in J. apply J.
+        eapply in_getBlockLocs__in_getBlocksLocs in H; eauto.
+        simpl. apply in_or_app. right. 
+        apply in_or_app. left. apply In_InCmdLocs; auto.
+      rewrite notin__lookupInsnViaIDFromBlock_none; auto.
+      eapply IHbs; eauto.
+Qed.
+
+Lemma find_promotable_alloca_spec: forall f cs nids pid ptyp pal,
+  find_promotable_alloca f cs nids = Some (pid, ptyp, pal) ->
+  exists pv, In (insn_alloca pid ptyp pv pal) cs /\
+             is_promotable f pid.
+Proof.
+  induction cs; simpl; intros.
+    congruence.
+
+    destruct a; try solve [apply IHcs in H; destruct H as [pv [H1 H2]]; eauto].
+    remember (is_promotable f i0 && negb (in_dec id_dec i0 nids)) as R.
+    destruct R; try solve [apply IHcs in H; destruct H as [pv [H1 H2]]; eauto].
+    inv H. 
+    symmetry in HeqR. apply andb_true_iff in HeqR. destruct HeqR.
+    eauto.
+Qed.
+
+Lemma WF_PhiInfo_spec1: forall pinfo, 
+  WF_PhiInfo pinfo -> 
+  uniqFdef (PI_f pinfo) ->
+  exists v, 
+    lookupInsnViaIDFromFdef (PI_f pinfo) (PI_id pinfo) = 
+      Some (insn_cmd 
+             (insn_alloca (PI_id pinfo) (PI_typ pinfo) v (PI_align pinfo))).
+Proof.
+  destruct pinfo. simpl.
+  intros.
+  destruct H as [H _].
+  unfold promotable_alloca in H.
+  remember (getEntryBlock PI_f0) as R.
+  destruct R; tinv H.
+  destruct b.
+  apply find_promotable_alloca_spec in H.
+  destruct H as [v [H _]].
+  exists v. 
+  symmetry in HeqR.
+  apply entryBlockInFdef in HeqR.
+  eapply IngetCmdsIDs__lookupCmdViaIDFromFdef in HeqR; eauto.
+  simpl in HeqR. auto.
+Qed.
+
+Definition is_promotable_fun pid := 
+  (fun acc b => 
+     let '(block_intro _ ps cs tmn) := b in
+     if (List.fold_left (fun re p => re || used_in_phi pid p) ps 
+          (used_in_tmn pid tmn)) then false
+     else
+       fold_left 
+         (fun acc0 c =>
+          if used_in_cmd pid c then
+            match c with
+            | insn_load _ _ _ _ => acc0
+            | insn_store _ _ v _ _ => negb (valueEqB v (value_id pid)) && acc0
+            | _ => false
+            end
+          else acc0) cs acc
+  ). 
+
+Lemma unused_in_phis__unused_in_phi: forall (pid id0 : id) (ps : phinodes)
+  (p0 : phinode) (J1 : ret p0 = lookupPhiNodeViaIDFromPhiNodes ps id0)
+  (J2 : fold_left (fun (re : bool) (p : phinode) => re || used_in_phi pid p) 
+          ps false = false),
+  used_in_phi pid p0 = false.
+Proof.
+  induction ps; simpl; intros.
+    congruence.
+
+    assert (fold_left (fun (re : bool) (p : phinode) => re || used_in_phi pid p)
+              ps false = false /\ used_in_phi pid a = false) as J3.
+      admit.
+    destruct J3 as [J3 J4].
+    destruct (getPhiNodeID a == id0); subst; eauto.
+      inv J1. auto.
+Qed.
+
+Lemma unused_in_cmds__unused_in_cmd: forall (pid id0 : id) (cs : cmds)
+  (c0 : cmd) (J1 : ret c0 = lookupCmdViaIDFromCmds cs id0)
+  (J2 : fold_left 
+          (fun acc0 c =>
+           if used_in_cmd pid c then
+             match c with
+             | insn_load _ _ _ _ => acc0
+             | insn_store _ _ v _ _ => negb (valueEqB v (value_id pid)) && acc0
+             | _ => false
+             end
+           else acc0) cs true = true),
+  match c0 with
+  | insn_load _ _ _ _ => True
+  | insn_store _ _ v _ _ => negb (valueEqB v (value_id pid)) 
+  | _ => used_in_cmd pid c0 = false
+  end.
+Proof.
+  induction cs; simpl; intros.
+    congruence.
+
+    assert (
+      fold_left 
+        (fun acc0 c =>
+         if used_in_cmd pid c then
+           match c with
+           | insn_load _ _ _ _ => acc0
+           | insn_store _ _ v _ _ => negb (valueEqB v (value_id pid)) && acc0
+           | _ => false
+           end
+         else acc0) cs true = true /\
+      (if used_in_cmd pid a then
+         match a with
+         | insn_load _ _ _ _ => true
+         | insn_store _ _ v _ _ => negb (valueEqB v (value_id pid)) && true
+         | _ => false
+         end
+       else true) = true) as J3.
+      admit.
+    destruct J3 as [J3 J4]. clear J2.
+    destruct (eq_atom_dec id0 (getCmdLoc a)); subst.
+      inv J1. clear IHcs J3.
+      remember (used_in_cmd pid a) as R.
+      destruct R.    
+        destruct a; auto.
+          apply andb_true_iff in J4. 
+          destruct J4; auto.
+        destruct a; auto.
+          simpl in *.
+          symmetry in HeqR.
+          apply orb_false_iff in HeqR. 
+           destruct HeqR. 
+           unfold valueEqB. 
+           destruct v; inv H; simpl.
+             destruct (value_dec (value_id i1) (value_id pid)); auto.
+             inversion e. subst.
+             destruct (id_dec pid pid); subst; inv H2; try congruence.
+         
+             destruct (value_dec (value_const c) (value_id pid)); auto.
+               congruence.
+      clear J4.
+      eapply IHcs in J3; eauto.
+Qed.
+
+Lemma is_promotable_spec: forall pid id0 instr bs,
+  fold_left (is_promotable_fun pid) bs true = true ->
+  lookupInsnViaIDFromBlocks bs id0 = ret instr ->
+  match instr with
+  | insn_cmd c0 =>
+    match c0 with
+    | insn_load _ _ _ _ => True
+    | insn_store _ _ v _ _ => negb (valueEqB v (value_id pid)) 
+    | _ => used_in_cmd pid c0 = false
+    end
+  | _ => used_in_insn pid instr = false
+  end.
+Proof.
+  induction bs; simpl; intros.
+    congruence.
+
+    assert (fold_left (is_promotable_fun pid) bs true = true /\ 
+            is_promotable_fun pid true a = true) as J.
+      admit.
+    destruct J as [J1 J2].
+    remember (lookupInsnViaIDFromBlock a id0) as R.
+    destruct R.
+      inv H0.
+      clear - J2 HeqR.
+      destruct a; simpl in *.
+      remember (fold_left
+                 (fun (re : bool) (p : phinode) => re || used_in_phi pid p) p
+                 (used_in_tmn pid t)) as R.
+      destruct R; tinv J2.
+      assert (fold_left 
+               (fun (re : bool) (p : phinode) => re || used_in_phi pid p) 
+                 p false = false /\
+              used_in_tmn pid t = false) as J.
+        admit.
+      destruct J as [J3 J4]. clear HeqR0.
+      remember (lookupPhiNodeViaIDFromPhiNodes p id0) as R1.
+      remember (lookupCmdViaIDFromCmds c id0) as R2.
+      destruct R1.
+        inv HeqR.
+        clear - J3 HeqR1. simpl.
+        eapply unused_in_phis__unused_in_phi in J3; eauto.
+
+        destruct R2; inv HeqR.
+        clear - J2 HeqR2. simpl.
+        eapply unused_in_cmds__unused_in_cmd in J2; eauto.
+
+      apply IHbs in H0; auto.
+Qed.
+
+Lemma WF_PhiInfo_spec3: forall pinfo, 
+  WF_PhiInfo pinfo -> 
+  forall instr id0, 
+    lookupInsnViaIDFromFdef (PI_f pinfo) id0 = Some instr ->
+    match instr with
+    | insn_cmd c0 =>
+      match c0 with
+      | insn_load _ _ _ _ => True
+      | insn_store _ _ v _ _ => negb (valueEqB v (value_id (PI_id pinfo))) 
+      | _ => used_in_cmd (PI_id pinfo) c0 = false
+      end
+    | _ => used_in_insn (PI_id pinfo) instr = false
+    end.
+Proof.
+  destruct pinfo. simpl.
+  intros.
+  destruct H as [H _].
+  unfold promotable_alloca in H.
+  remember (getEntryBlock PI_f0) as R.
+  destruct R; tinv H.
+  destruct b.
+  apply find_promotable_alloca_spec in H.
+  destruct H as [v [_ H]].
+  destruct PI_f0. simpl in *.
+  eapply is_promotable_spec in H0; eauto.
+Qed.
+
+Definition valueInInsnOperands (v0:value) (instr:insn) : Prop :=
+match instr with
+| insn_phinode (insn_phi _ _ ls) => 
+    In v0 (list_prj1 _ _ (unmake_list_value_l ls))
+| insn_cmd c => valueInCmdOperands v0 c
+| insn_terminator tmn => valueInTmnOperands v0 tmn
+end.
+
+Lemma used_in_phi__wf_use_at_head: forall pinfo v0 (p : phinode)
+  (H0 : used_in_phi (PI_id pinfo) p = false)
+  (H1 : valueInInsnOperands v0 (insn_phinode p)),
+  wf_use_at_head pinfo v0.
+Proof.
+  intros.
+  unfold wf_use_at_head.
+  destruct p; simpl in *.
+  induction l0; tinv H1.
+    simpl in *.
+    apply orb_false_iff in H0.
+    destruct H0 as [J1 J2].
+    destruct H1 as [H1 | H1]; subst; auto.
+Qed.
+
+Lemma WF_PhiInfo_spec4: forall pinfo, 
+  WF_PhiInfo pinfo -> 
+  forall instr id0 v0, 
+    lookupInsnViaIDFromFdef (PI_f pinfo) id0 = Some instr ->
+    match instr with
+    | insn_cmd c0 =>
+      match c0 with
+      | insn_load _ _ _ _ => False
+      | insn_store _ _ v _ _ => v = v0 
+      | _ => valueInCmdOperands v0 c0
+      end
+    | _ => valueInInsnOperands v0 instr
+    end ->
+    wf_use_at_head pinfo v0.
+Proof.
+  intros.
+  apply WF_PhiInfo_spec3 in H0; auto.
+  destruct instr.
+    simpl in H0. 
+    eapply used_in_phi__wf_use_at_head in H1; eauto.
+
+    unfold wf_use_at_head.
+    destruct c; tinv H1; simpl in *;
+      try solve [
+        subst; auto |
+        match goal with
+        | H0 : used_in_value _ ?v1 || used_in_value _ ?v2 = false,
+          H1 : ?v0 = ?v1 \/ ?v0 = ?v2 |- _ =>
+            apply orb_false_iff in H0;
+            destruct H0 as [J1 J2];
+            destruct H1; subst; auto
+        end
+      ].
+
+      subst. 
+      destruct v0; auto.
+      unfold valueEqB in H0.  
+      destruct (value_dec (value_id i1) (value_id (PI_id pinfo))); simpl in *.
+        congruence.
+
+        destruct (id_dec i1 (PI_id pinfo)); subst; auto.
+          congruence.
+
+      admit. 
+      admit.
+      admit. 
+
+    unfold wf_use_at_head.
+    destruct t; simpl in *; subst; 
+      try solve [auto | match goal with
+                        | H1: False |- _ => inv H1
+                        end].
+Qed.
+
+Lemma WF_PhiInfo_spec5: forall pinfo pn b, 
+  WF_PhiInfo pinfo -> 
+  phinodeInFdefBlockB pn (PI_f pinfo) b = true -> 
+  used_in_phi (PI_id pinfo) pn = false.
+Proof.
+  intros.
+Admitted.
+
+Lemma WF_PhiInfo_spec6: forall pinfo l' ps' cs' tmn', 
+  WF_PhiInfo pinfo -> 
+  ret block_intro l' ps' cs' tmn' = lookupBlockViaLabelFromFdef (PI_f pinfo) l' ->
+  ~ In (PI_id pinfo) (getPhiNodesIDs ps').
+Admitted.
+
+Lemma PhiInfo_must_be_promotable_alloca: forall pinfo l0 ps0 cs1 c cs2 tmn0,
+  WF_PhiInfo pinfo ->
+  uniqFdef (PI_f pinfo) ->
+  getCmdLoc c = PI_id pinfo ->
+  (forall id1 typ1 v1 al1, c <> insn_alloca id1 typ1 v1 al1) ->
+  blockInFdefB (block_intro l0 ps0 (cs1++c::cs2) tmn0) (PI_f pinfo) = true ->
+  False. 
+Proof.
+  intros.
+  eapply IngetCmdsIDs__lookupCmdViaIDFromFdef in H3; eauto using in_middle.
+  apply WF_PhiInfo_spec1 in H; auto.
+  destruct H as [v' H].
+  simpl in H3. rewrite H1 in H3. rewrite H3 in H. inv H.
+  assert (W:=@H2 (PI_id pinfo) (PI_typ pinfo) v' (PI_align pinfo)).
+  auto.
 Qed.
 
 Lemma preservation_return : forall maxb pinfo (HwfPI : WF_PhiInfo pinfo)  
@@ -967,10 +1271,6 @@ Local Opaque inscope_of_tmn inscope_of_cmd.
     SSSCase "sdom".
 
     destruct (fdef_dec (PI_f pinfo) F'); subst; auto.
-    unfold inscope_of_pc in Hinscope2.
-    remember (inscope_of_cmd 
-      (PI_f pinfo) (block_intro l2 ps2 (cs2' ++ c' :: cs') tmn') c') as R2.
-    destruct R2; try solve [inversion Hinscope2].
 
     remember (getCmdID c') as R.
     destruct c'; try solve [inversion H].
@@ -993,17 +1293,12 @@ Local Opaque inscope_of_tmn inscope_of_cmd.
       apply NoDup_split in Hdisjals'.
       destruct Hdisjals'; auto.
     eapply free_allocas_preserves_wf_defs in Hinscope2; eauto. clear Hnodup.
-    unfold inscope_of_pc.
     destruct cs'.
     SSSSCase "cs' = nil".
       assert (~ In (getCmdLoc (insn_call i0 n c t v p)) (getCmdsLocs cs2')) 
         as Hnotin.
         eapply preservation_helper1; eauto.
 
-      assert (HeqR2':=HeqR2).
-      apply inscope_of_cmd_tmn in HeqR2; auto.
-      destruct HeqR2 as [ids2 [J1 J2]].
-      simpl_env. rewrite <- J1.
       unfold Opsem.returnUpdateLocals in H1. simpl in H1.
       remember (Opsem.getOperandValue (los,nts) Result lc gl) as R1.
       destruct R1; try solve [inv H1].
@@ -1014,28 +1309,23 @@ Local Opaque inscope_of_tmn inscope_of_cmd.
 
         remember (MDGVs.lift_op1 (fit_gv (los, nts) t) g t) as R2.
         destruct R2; inv H1.
-
-        apply wf_defs_updateAddAL with (ids1:=l0); auto.
+        apply wf_defs_updateAddAL; auto.
           split.
             eapply preservation_return_helper; eauto; simpl; auto.
 
             intro; subst.
-            admit. (* PI_id pinfo cannot be of an id for callsite *) 
-
+            clear - HwfPI HBinF2 HuniqF.
+            apply PhiInfo_must_be_promotable_alloca in HBinF2; 
+              try solve [auto | inv HBinF2 | intros; congruence].
+ 
       SSSSSCase "c' defines nothing".
-        destruct n; inv HeqR. inv H1.
-        simpl in J2.
-        eapply wf_defs_eq; eauto. 
+        destruct n; inv HeqR. inv H1. auto.
         
     SSSSCase "cs' <> nil".
       assert (NoDup (getCmdsLocs (cs2' ++ [insn_call i0 n c t v p] ++ [c0] ++ 
         cs'))) as Hnodup.
         eapply preservation_helper2; eauto.
 
-      assert (HeqR2':=HeqR2). simpl_env in HeqR2.
-      apply inscope_of_cmd_cmd in HeqR2; auto.
-      destruct HeqR2 as [ids2 [J1 J2]].        
-      simpl_env. rewrite <- J1.
       unfold Opsem.returnUpdateLocals in H1. simpl in H1.
       remember (Opsem.getOperandValue (los,nts) Result lc gl) as R1.
       destruct R1; try solve [inv H1].
@@ -1047,17 +1337,17 @@ Local Opaque inscope_of_tmn inscope_of_cmd.
         destruct R2; inv H1.
         inv Hwfc. inv H16. inv H7. inv H18.
 
-        apply wf_defs_updateAddAL with (ids1:=l0); auto.
+        apply wf_defs_updateAddAL; auto.
           split.
             eapply preservation_return_helper; eauto; simpl; auto.
 
             intro; subst.
-            admit. (* PI_id pinfo cannot be of an id for callsite *) 
+            clear - HwfPI HBinF2 HuniqF.
+            apply PhiInfo_must_be_promotable_alloca in HBinF2; 
+              try solve [auto | inv HBinF2 | intros; congruence].
 
       SSSSSCase "c' defines nothing".
-        destruct n; inv HeqR. inv H1.
-        simpl in J2.
-        eapply wf_defs_eq; eauto. 
+        destruct n; inv HeqR. inv H1. auto.
 
       SSSCase "wflc".
         clear - Hwflc1 Hwflc2 H1 Hwfg HwfM H0.
@@ -1090,14 +1380,11 @@ Definition wf_GVs_in_ECs (maxb:Values.block) (pinfo:PhiInfo) TD M
   (head:Opsem.ExecutionContext) tail (id1:id)(gv1:GVsT DGVs) : Prop :=
 let '(Opsem.mkEC f b cs tmn lc als) := head in
 (if (fdef_dec (PI_f pinfo) f) then 
-  forall ids0, 
-    inscope_of_pc f b cs tmn = Some ids0 ->
-    wf_defs maxb pinfo TD M lc ids0 als ->
-    wf_GVs maxb pinfo TD M lc ids0 als id1 gv1
+    wf_defs maxb pinfo TD M lc als ->
+    wf_GVs maxb pinfo TD M lc als id1 gv1
 else True) /\
 (forall ec0 (Hin : In ec0 tail) (gvsa : GVsT DGVs) 
-    (Heq : Opsem.CurFunction ec0 = PI_f pinfo) ids0
-    (Hscp: inscope_of_EC ec0 = Some ids0) (Hin1: In (PI_id pinfo) ids0)
+    (Heq : Opsem.CurFunction ec0 = PI_f pinfo) 
     (Hlkup : lookupAL (GVsT DGVs) (Opsem.Locals ec0) (PI_id pinfo) = ret gvsa),
     no_alias gv1 gvsa) /\
 (valid_ptrs (Mem.nextblock M) gv1).
@@ -1152,78 +1439,31 @@ Local Opaque inscope_of_cmd inscope_of_tmn.
     split.
     SSCase "wf_EC".
     split.
-    SSSCase "sdom".
-    destruct (fdef_dec (PI_f pinfo) F); subst; auto.
-
-  unfold inscope_of_pc in *.
-  remember (inscope_of_cmd (PI_f pinfo) 
-    (block_intro l1 ps1 (cs1' ++ c0 :: cs) tmn) c0) as R1. 
-  assert (HeqR1':=HeqR1).
-
-Transparent inscope_of_cmd.
-
-  unfold inscope_of_cmd, inscope_of_id in HeqR1'.
-  destruct R1; try solve [inversion Hinscope1].
-  repeat (split; try solve [auto]).
-      assert (Hid':=Hid).
-      symmetry in Hid.
-      apply getCmdLoc_getCmdID in Hid.
-      subst.
-      destruct cs; simpl_env in *.
-      SSSSCase "cs = nil".
-        assert (~ In (getCmdLoc c0) (getCmdsLocs cs1')) as Hnotin.
-          (* this lemma should be lifted to the top *)
-          eapply preservation_helper1; eauto.
-
-        apply inscope_of_cmd_tmn in HeqR1; auto.
-        destruct HeqR1 as [ids2 [J1 J2]].        
-        rewrite <- J1.
-        assert (In c0 (cs1' ++ [c0])) as HinCs.
-          apply in_or_app. right. simpl. auto.
-        assert (Hwfc := HBinF1).
-        eapply wf_system__wf_cmd with (c:=c0) in Hwfc; 
-          eauto.
-        rewrite <- Hid' in J2.
-        assert (HwfF:=HFinPs1). eapply wf_system__wf_fdef in HwfF; eauto.
-        eapply wf_defs_updateAddAL; eauto.
-
-      SSSSCase "cs <> nil".
-        assert (NoDup (getCmdsLocs (cs1' ++ [c0] ++ [c] ++ cs))) as Hnodup.
-          (* this lemma should be lifted to the top *)
-          eapply preservation_helper2; eauto.
-
-        apply inscope_of_cmd_cmd in HeqR1; auto.
-        destruct HeqR1 as [ids2 [J1 J2]].        
-        rewrite <- J1.
-        assert (In c0 (cs1' ++ [c0] ++ [c] ++ cs)) as HinCs.
-          apply in_or_app. right. simpl. auto.
-        assert (Hwfc := HBinF1).
-        eapply wf_system__wf_cmd with (c:=c0) in Hwfc; 
-          eauto.
-        rewrite <- Hid' in J2.
-        assert (HwfF:=HFinPs1). eapply wf_system__wf_fdef in HwfF; eauto.
-        eapply wf_defs_updateAddAL; eauto.
+      SSSCase "sdom".
+      destruct (fdef_dec (PI_f pinfo) F); subst; auto.
+      eapply wf_defs_updateAddAL; eauto.
 
       SSSCase "wflc".
-        apply updateAddAL__wf_lc; auto.
+      apply updateAddAL__wf_lc; auto.
 
     split; auto.
     SSCase "wf_ECs_head_tail".
       eapply updateAddAL__wf_ECStack_head_tail; eauto.
-Transparent inscope_of_cmd inscope_of_tmn.
-
 Qed.
 
 Lemma BOP__wf_GVs_in_ECs : forall (v : value) (v0 : value) (id1 : id) (bop0 : bop)
-  gvs3 TD bop0 sz0 lc gl hd tl Mem0 td pinfo maxb (Hneq: id1 <> PI_id pinfo)
+  gvs3 TD bop0 sz0 lc gl hd tl Mem0 td pinfo maxb 
+  (Hneq: PI_f pinfo = Opsem.CurFunction hd -> id1 <> PI_id pinfo)
   (H11 : BOP TD lc gl bop0 sz0 v v0 = ret gvs3),
   wf_GVs_in_ECs maxb pinfo td Mem0 hd tl id1 gvs3.
 Proof.
   intros. 
-  unfold wf_GVs_in_ECs. destruct hd.
-  split.
+  unfold wf_GVs_in_ECs. destruct hd; simpl in *.
+  split.   
     destruct (fdef_dec (PI_f pinfo) CurFunction); subst; auto.
     intros.
+    assert (PI_f pinfo = PI_f pinfo) as EQ. auto.
+    apply Hneq in EQ. clear Hneq.
     split; intros; subst; try congruence.
       eapply BOP_preserves_no_alias; eauto.
   split.
@@ -1237,8 +1477,7 @@ Lemma operand__no_alias_with__tail': forall maxb gl (Hwfgl : wf_globals maxb gl)
   (tl : list Opsem.ExecutionContext) pinfo Mem
   (Hwfstk : wf_ECStack_head_tail maxb pinfo TD Mem lc tl)
   (ec0 : Opsem.ExecutionContext) (Hin: In ec0 tl) (gvsa : GVsT DGVs)
-  (Heq: Opsem.CurFunction ec0 = PI_f pinfo) ids0
-  (Hscp: inscope_of_EC ec0 = ret ids0) (Hin: In (PI_id pinfo) ids0)
+  (Heq: Opsem.CurFunction ec0 = PI_f pinfo)
   (Hlkup: lookupAL (GVsT DGVs) (Opsem.Locals ec0) (PI_id pinfo) = ret gvsa),
   no_alias gv1 gvsa.
 Proof.
@@ -1250,12 +1489,9 @@ Lemma CAST__wf_GVs_in_ECs : forall (v : value) (id1 : id)
   gvs2 TD gl EC Mem pinfo maxb castop0 t1 t2 
   (Hwflc: wf_lc Mem (@Opsem.Locals DGVs EC)) 
   (Hwfgl: wf_globals maxb gl) (HwfM: maxb < Mem.nextblock Mem)
-  (Hwfv: forall ids0,
-         let '(Opsem.mkEC F B cs tmn _ _) := EC in
-         F = (PI_f pinfo) ->
-         inscope_of_pc F B cs tmn = Some ids0 ->
-         wf_use_at_head pinfo ids0 v)
-  (Hneq: id1 <> PI_id pinfo)
+  (Hwfv: Opsem.CurFunction EC = (PI_f pinfo) ->
+         wf_use_at_head pinfo v)
+  (Hneq: PI_f pinfo = Opsem.CurFunction EC -> id1 <> PI_id pinfo)
   (H11 : Opsem.CAST TD (@Opsem.Locals DGVs EC) gl castop0 t1 v t2 
            = ret gvs2) tl
   (Hwfstk: 
@@ -1270,10 +1506,9 @@ Proof.
   split.
     destruct (fdef_dec (PI_f pinfo) CurFunction); subst; auto.
     intros.
+    assert (PI_f pinfo = PI_f pinfo) as EQ. auto.
+    apply Hneq in EQ. clear Hneq.
     split; intros; subst; try congruence.
-      assert (H2':=H2).
-      apply H0 in H2; auto.
-      destruct H2 as [[J5 [J6 J3]] J4]; eauto.
       eapply operand__no_alias_with__head with (als:=Allocas) (mptr0:=gv1)
         (M:=Mem) in J1; eauto.
         clear - J1 J2. 
@@ -1297,7 +1532,8 @@ Admitted.
 
 Lemma mload__wf_GVs_in_ECs : forall (v : value) (v0 : value) (id1 : id) 
   gvs3 t align0 EC Mem td pinfo maxb mp
-  (Hneq: id1 <> PI_id pinfo) (HwfM: wf_Mem maxb td Mem)
+  (Hneq: PI_f pinfo = Opsem.CurFunction EC -> id1 <> PI_id pinfo) 
+  (HwfM: wf_Mem maxb td Mem)
   (H1 : mload td Mem mp t align0 = ret gvs3) tl
   (Hwfstk: wf_ECStack_head_tail maxb pinfo td Mem (Opsem.Locals EC) tl),
   wf_GVs_in_ECs maxb pinfo td Mem EC tl id1 gvs3.
@@ -1307,9 +1543,11 @@ Proof.
   split.
     destruct (fdef_dec (PI_f pinfo) CurFunction); subst; auto.
     intros.
+    assert (PI_f pinfo = PI_f pinfo) as EQ. auto.
+    apply Hneq in EQ. clear Hneq.
     split; intros; subst; try congruence.
-      apply H0 in H3; auto.
-      destruct H3 as [[J1 [J2 J3]] _]; eauto.
+      apply H in H0; auto.
+      destruct H0 as [[J1 [J2 J3]] _]; eauto.
   split.
     intros. simpl in Hwfstk. apply Hwfstk in Hin.
     destruct ec0. simpl in *.
@@ -1371,13 +1609,10 @@ Lemma GEP__wf_GVs_in_ECs : forall (v : value) (v0 : value) (id1 : id)
   mp' TD t gl EC Mem pinfo maxb (mp:GVsT DGVs) mps 
   inbounds0 vidxs (Hwflc: wf_lc Mem (@Opsem.Locals DGVs EC)) 
   (Hwfgl: wf_globals maxb gl) (HwfM: maxb < Mem.nextblock Mem)
-  (Hwfv: forall ids0,
-         let '(Opsem.mkEC F B cs tmn _ _) := EC in
-         F = (PI_f pinfo) ->
-         inscope_of_pc F B cs tmn = Some ids0 ->
-         wf_use_at_head pinfo ids0 v)
+  (Hwfv: PI_f pinfo = Opsem.CurFunction EC -> 
+         wf_use_at_head pinfo v)
   (H : Opsem.getOperandValue TD v (Opsem.Locals EC) gl = ret mps)
-  (H0 : mp @ mps) (Hneq: id1 <> PI_id pinfo)
+  (H0 : mp @ mps)(Hneq: PI_f pinfo = Opsem.CurFunction EC -> id1 <> PI_id pinfo)
   (H1 : Opsem.GEP TD t mp vidxs inbounds0 = ret mp') tl
   (Hwfstk: wf_ECStack_head_tail maxb pinfo TD Mem (Opsem.Locals EC) tl),
   wf_GVs_in_ECs maxb pinfo TD Mem EC tl id1 mp'.
@@ -1387,10 +1622,12 @@ Proof.
   split.
     destruct (fdef_dec (PI_f pinfo) CurFunction); subst; auto.
     intros.
+    assert (PI_f pinfo = PI_f pinfo) as EQ. auto.
+    apply Hneq in EQ. clear Hneq.
     split; intros; subst; try congruence.
-      assert (H5':=H5).
-      apply H3 in H5; auto.
-      destruct H5 as [[J1 [J2 J3]] J4]; eauto.
+     assert (H3':=H3).
+     apply H2 in H3; auto.
+      destruct H3 as [[J1 [J2 J3]] J4]; eauto.
       eapply operand__no_alias_with__head with (als:=Allocas) (mptr0:=mp)
         (M:=Mem) in H; eauto.
         clear - H1 H. 
@@ -1467,12 +1704,32 @@ Proof.
         intros. apply Hwf. simpl. auto.
 Qed.
 
-Lemma in_params__used: forall id1 A (lp : list (A * value)) (t1 : A),
+Lemma fold_left_or_spec : forall B (f:bool -> B -> bool)
+  (J:forall a b, a = true -> f a b = true), 
+  forall (l1:list B), List.fold_left f l1 true = true.
+Proof.
+  induction l1; simpl; intros; eauto.
+    rewrite J; auto.
+Qed.
+
+Lemma in_params__used: forall id1 A (t1 : A) (lp : list (A * value)) init,
   fold_left
     (fun (acc : bool) (p : A * value) =>
-     let '(_, v) := p in used_in_value id1 v || acc) lp false ->
+     let '(_, v) := p in used_in_value id1 v || acc) lp init = false ->
   ~ In (t1, value_id id1) lp.
-Admitted.
+Proof.
+  induction lp as [|[]]; simpl; intros; auto.
+    intro J.
+    destruct J as [J | J].
+      inv J.
+      simpl in H.
+      destruct (id_dec id1 id1); try congruence.
+      simpl in H.
+      rewrite fold_left_or_spec in H; try congruence.
+        intros. subst. destruct b. apply orb_true_iff; auto.
+
+      apply IHlp in H. congruence.
+Qed.
 
 Lemma initLocals_preserves_wf_ECStack_head_tail: forall Mem (lc:DGVMap) maxb TD 
   ECs lc' gl (Hwflc1 : wf_lc Mem lc) pinfo gvs la lp EC
@@ -1480,18 +1737,14 @@ Lemma initLocals_preserves_wf_ECStack_head_tail: forall Mem (lc:DGVMap) maxb TD
     PI_f pinfo = Opsem.CurFunction EC ->
     List.fold_left 
       (fun acc p => let '(_, v):=p in used_in_value (PI_id pinfo) v || acc) 
-      lp false)
+      lp false = false)
   (Hwfg : wf_globals maxb gl)
   (H3 : Opsem.params2GVs TD lp lc gl = ret gvs)
   (H4 : Opsem.initLocals TD la gvs = ret lc')
   (Heq2 : lc = Opsem.Locals EC)
   (Hfr2 : wf_ECStack_head_tail maxb pinfo TD Mem lc ECs)
   (Hscp: if fdef_dec (PI_f pinfo) (Opsem.CurFunction EC) then
-           match inscope_of_EC EC with
-           | ret ids0 => 
-             wf_defs maxb pinfo TD Mem (Opsem.Locals EC) ids0 (Opsem.Allocas EC)
-           | merror => False
-           end
+           wf_defs maxb pinfo TD Mem (Opsem.Locals EC) (Opsem.Allocas EC)
          else True),
   wf_ECStack_head_tail maxb pinfo TD Mem lc' (EC :: ECs).
 Proof.
@@ -1501,9 +1754,8 @@ Proof.
     unfold wf_ECStack_head_in_tail. destruct ec0. simpl in *.
     intros.
     destruct (fdef_dec (PI_f pinfo) CurFunction); subst; try congruence.    
-    rewrite H0 in Hscp.
-    apply_clear Hscp in H2.
-    destruct H2 as [[[mb [J11 [J14 J15]]] [J12 J13]] J2]; subst.
+    apply_clear Hscp in H0.
+    destruct H0 as [[[mb [J11 [J14 J15]]] [J12 J13]] J2]; subst.
     split; eauto.
     split; intros; eauto.
       eapply initializeFrameValues_preserves_no_alias in H4; eauto.
@@ -1511,14 +1763,14 @@ Proof.
         omega.
 
         intros.
-        apply J2 in H6. unfold wf_non_alloca_GVs in H6.
+        apply J2 in H2. unfold wf_non_alloca_GVs in H2.
         destruct (id_dec id0 (PI_id pinfo)); subst; auto.
-          contradict H5. eapply in_params__used; eauto.
+          contradict H1. eapply in_params__used; eauto.
 
     destruct ec0. simpl.
-    intros ids0 gvsa Heq Hscp' Hin' Hlkup.
-    apply_clear Hfr2 in Hin. simpl in Hin. eapply_clear Hin in Hscp'. 
-    destruct Hscp' as [[mb [J11 J12]] [J2 J3]]; subst.
+    intros gvsa Heq Hlkup.
+    apply_clear Hfr2 in Hin. simpl in Hin. eapply_clear Hin in Hlkup. 
+    destruct Hlkup as [[mb [J11 J12]] [J2 J3]]; subst.
     split; eauto.
     split; auto.
       intros.
@@ -1526,15 +1778,65 @@ Proof.
       eapply params2GVs_preserves_no_alias; eauto. omega.
 Qed.
 
+Lemma IngetArgsIDs__lookupCmdViaIDFromFdef: forall fa rt fid la va lb id0
+  (Huniq: uniqFdef (fdef_intro (fheader_intro fa rt fid la va) lb))
+  (H0 : In id0 (getArgsIDs la)),
+  lookupInsnViaIDFromFdef (fdef_intro (fheader_intro fa rt fid la va) lb) id0 
+    = None.
+Admitted.
+
+Lemma In_initializeFrameValues__In_getArgsIDs: forall (GVsSig : GenericValues) 
+  (TD : TargetData) (la : args) (gvs : list (GVsT GVsSig)) (id1 : atom) 
+  (lc : Opsem.GVsMap) (gv : GVsT GVsSig) acc,
+  Opsem._initializeFrameValues TD la gvs acc = ret lc ->
+  lookupAL (GVsT GVsSig) lc id1 = ret gv -> 
+  In id1 (getArgsIDs la) \/ id1 `in` dom acc.
+Proof.
+  induction la as [|[]]; simpl; intros.
+    inv H.
+    right. apply lookupAL_Some_indom in H0; auto.
+
+    destruct p.
+    destruct gvs.
+      inv_mbind'.
+      destruct (id_dec i0 id1); subst; auto.
+      rewrite <- lookupAL_updateAddAL_neq in H0; auto.
+      eapply IHla in H0; eauto.
+      destruct H0 as [H0 | H0]; auto.
+
+      inv_mbind'.
+      destruct (id_dec i0 id1); subst; auto.
+      rewrite <- lookupAL_updateAddAL_neq in H0; auto.
+      eapply IHla in H0; eauto.
+      destruct H0 as [H0 | H0]; auto.
+Qed.
+
+Lemma In_initLocals__In_getArgsIDs : forall GVsSig TD la gvs id1 lc gv,
+  @Opsem.initLocals GVsSig TD la gvs = Some lc ->
+  lookupAL _ lc id1 = Some gv ->
+  In id1 (getArgsIDs la).
+Proof.
+  unfold Opsem.initLocals.
+  intros.
+  eapply In_initializeFrameValues__In_getArgsIDs in H; eauto.
+  destruct H as [H | H]; auto.
+    fsetdec.
+Qed.
+
 Lemma initLocals_preserves_wf_defs : forall fid fa rt la va lb gvs 
   lc Mem TD pinfo maxb (Hwfpi: WF_PhiInfo pinfo)
   (Huniq: uniqFdef (fdef_intro (fheader_intro fa rt fid la va) lb))
   (Hinit : Opsem.initLocals TD la gvs = Some lc) 
   (Heq: fdef_intro (fheader_intro fa rt fid la va) lb = PI_f pinfo),
-  wf_defs maxb pinfo TD Mem lc (getArgsIDs la) nil.
+  wf_defs maxb pinfo TD Mem lc nil.
 Proof.
-  intros. intros gvsa Hin Hlkup.
-  admit. (* promotable allocas cannot be arguments *)
+  intros. intros gvsa Hlkup.
+  eapply In_initLocals__In_getArgsIDs in Hinit; eauto.
+  eapply IngetArgsIDs__lookupCmdViaIDFromFdef in Hinit; eauto.
+  rewrite Heq in *.
+  apply WF_PhiInfo_spec1 in Huniq; auto.
+  destruct Huniq as [v Huniq].
+  rewrite Huniq in Hinit. congruence.
 Qed.
 
 Lemma params2GVs_preserves_wf_lc: forall maxb gl M
@@ -1688,12 +1990,12 @@ Lemma mstore_preserves_wf_defs_at_head : forall maxb pinfo TD M
   (Hgetop: Opsem.getOperandValue TD v lc gl = ret gvs1)
   (Hinp: mp2 @ mps2) (Hin: gv1 @ gvs1) (Hwfgl: wf_globals maxb gl)
   (Hst: mstore TD M mp2 t gv1 align = Some M')
-  ids0 (Hwfu: wf_use_at_head pinfo ids0 v) 
-  (Hwf: wf_defs maxb pinfo TD M lc ids0 als),
-  wf_defs maxb pinfo TD M' lc ids0 als.
+  (Hwfu: wf_use_at_head pinfo v) 
+  (Hwf: wf_defs maxb pinfo TD M lc als),
+  wf_defs maxb pinfo TD M' lc als.
 Proof.
   intros. unfold wf_defs. 
-  intros gvsa Hpindom Hlkp.
+  intros gvsa Hlkp.
   assert (no_alias gv1 gvsa) as J.
     eapply operand__no_alias_with__head with (mptrs:=gvs1); eauto.
   assert (Hlkp':=Hlkp).
@@ -1722,12 +2024,11 @@ Lemma mstore_preserves_wf_defs_in_tail : forall maxb pinfo TD M
   (Heq1: Opsem.CurFunction EC = PI_f pinfo)
   (Heq2: Opsem.Locals EC = lc2) 
   (Hht: wf_ECStack_head_in_tail maxb pinfo TD M lc1 EC)
-  ids0 (Hscp: inscope_of_EC EC = ret ids0) 
-  (Hwf: wf_defs maxb pinfo TD M lc2 ids0 als),
-  wf_defs maxb pinfo TD M' lc2 ids0 als.
+  (Hwf: wf_defs maxb pinfo TD M lc2 als),
+  wf_defs maxb pinfo TD M' lc2 als.
 Proof.
   intros. unfold wf_defs. 
-  intros gvsa Hpindom Hlkp.
+  intros gvsa Hlkp.
   assert (Hlkp':=Hlkp).
   apply Hwf in Hlkp'; auto.
   destruct Hlkp' as [J1 J2].
@@ -1903,12 +2204,12 @@ Qed.
 
 Lemma malloc_preserves_wf_defs_in_tail : forall maxb pinfo TD M  
   M' als lc mb align0 gn tsz (Hal: malloc TD M tsz gn align0 = ret (M', mb))
-  ids0 (Hwf: wf_defs maxb pinfo TD M lc ids0 als),
-  wf_defs maxb pinfo TD M lc ids0 als ->
-  wf_defs maxb pinfo TD M' lc ids0 als.
+  (Hwf: wf_defs maxb pinfo TD M lc als),
+  wf_defs maxb pinfo TD M lc als ->
+  wf_defs maxb pinfo TD M' lc als.
 Proof.
   intros. unfold wf_defs. 
-  intros gvsa Hpindom Hlkp.
+  intros gvsa Hlkp.
   assert (Hlkp':=Hlkp).
   apply Hwf in Hlkp'; auto.
   destruct Hlkp' as [J1 J2].
@@ -1985,12 +2286,10 @@ Lemma impure_cmd_updated_preserves_wf_EC : forall maxb pinfo TD M M' lc F B
   (HFinPs: InProductsB (product_fdef F) Ps = true)
   (HBinF: blockInFdefB B F = true) id0
   (Hid : getCmdID c0 = Some id0) gv3
-  (Hwfdefs: forall ids0,
-              F = (PI_f pinfo) ->
-              inscope_of_pc F B (c0::cs) tmn = Some ids0 ->
-              wf_defs maxb pinfo TD M lc ids0 als ->
+  (Hwfdefs:   F = (PI_f pinfo) ->
+              wf_defs maxb pinfo TD M lc als ->
               wf_defs maxb pinfo TD M' 
-                (updateAddAL (GVsT DGVs) lc id0 gv3) (id0::ids0) als')
+                (updateAddAL (GVsT DGVs) lc id0 gv3) als')
   (Hwflc: wf_lc M lc -> wf_lc M' (updateAddAL (GVsT DGVs) lc id0 gv3)) EC
   (Heq: EC = {| Opsem.CurFunction := F;
                Opsem.CurBB := B;
@@ -2011,48 +2310,6 @@ Proof.
   destruct HwfEC as [J1 J2].
   split; auto.
   destruct (fdef_dec (PI_f pinfo) F); subst; auto.
-  unfold inscope_of_pc in *.
-  remember (inscope_of_cmd (PI_f pinfo) 
-    (block_intro l1 ps1 (cs1' ++ c0 :: cs) tmn) c0) as R1. 
-  assert (HeqR1':=HeqR1).
-  unfold inscope_of_cmd, inscope_of_id in HeqR1'.
-
-  destruct R1; try solve [inversion J1].
-  repeat (split; try solve [auto]).
-      destruct cs; simpl_env in *.
-      SSSSCase "cs = nil".
-        assert (~ In (getCmdLoc c0) (getCmdsLocs cs1')) 
-          as Hnotin.
-          eapply preservation_helper1; eauto.
-
-        apply inscope_of_cmd_tmn in HeqR1; auto.
-        destruct HeqR1 as [ids2 [J1' J2']].
-        rewrite <- J1'.
-        assert (In c0 (cs1' ++ [c0])) as HinCs.
-          apply in_or_app. right. simpl. auto.
-        assert (Hwfc := HBinF).
-        eapply wf_system__wf_cmd with (c:=c0) in Hwfc; 
-          eauto.
-        assert (HwfF:=HFinPs). eapply wf_system__wf_fdef in HwfF; eauto.
-        rewrite Hid in J2'.
-        eapply wf_defs_eq; eauto.       
-
-      SSSSCase "cs <> nil".
-        assert (NoDup (getCmdsLocs (cs1' ++ [c0] ++ [c] ++ cs))) 
-          as Hnodup.
-          eapply preservation_helper2; eauto.
-
-        apply inscope_of_cmd_cmd in HeqR1; auto.
-        destruct HeqR1 as [ids2 [J1' J2']].        
-        rewrite <- J1'.
-        assert (In c0 (cs1' ++ [c0] ++ [c] ++ cs)) 
-          as HinCs.
-          apply in_or_app. right. simpl. auto.
-        assert (Hwfc := HBinF).
-        eapply wf_system__wf_cmd with (c:=c0) in Hwfc; 
-          eauto.
-        rewrite Hid in J2'. 
-        eapply wf_defs_eq; eauto.
 Qed.
 
 Lemma valid_ptrs__no_alias__fresh_ptr: forall bound TD mb t (Hbd: bound <= mb) 
@@ -2081,6 +2338,9 @@ Proof.
       intros. inv H.
 Admitted.
 
+(* The current design of malloc is incorrect! It must ensure that mload is
+   successful at the allocated address. To do so, malloc must ensure all 
+   subcomponents in an aggregated object are well-aligned! *)
 Lemma mload_aux_malloc_same': forall TD M M' mb align0 gn tsz mc
   (Hal : malloc TD M tsz gn align0 = ret (M', mb)),
   exists gvs1, mload_aux M' mc mb (Int.signed 31 (Int.repr 31 0)) = ret gvs1.
@@ -2090,24 +2350,29 @@ Proof.
   destruct Hal as [n [J1 [J2 J3]]].
 Admitted.
 
-Lemma alloca_preserves_wf_defs_at_head : forall maxb pinfo TD M  
-  M' gl als lc t v
-  (Hwfgl: wf_globals maxb gl) mb id0 tmn align0 cs cs1' l1 ps1 F gn tsz
-  (Hal: malloc TD M tsz gn align0 = ret (M', mb)) (HwfM: wf_Mem maxb TD M)
-  (Hwflc : wf_lc M lc) (Hsize: getTypeAllocSize TD t = ret tsz),
-  forall ids0,
+(* We need to restrict the wf_alloca rule *)
+Lemma WF_PhiInfo_spec2: forall pinfo ifs S los nts Ps,
+  WF_PhiInfo pinfo ->
+  wf_fdef ifs S (module_intro los nts Ps) (PI_f pinfo) ->
+  exists mc, flatten_typ (los, nts) (PI_typ pinfo) = Some mc.
+Admitted.
+
+Lemma alloca_preserves_wf_defs_at_head : forall maxb pinfo los nts M  
+  M' gl als lc t 
+  (Hwfpi : WF_PhiInfo pinfo) ifs S Ps
+  (HwfF: wf_fdef ifs S (module_intro los nts Ps) (PI_f pinfo))
+  (Hwfgl: wf_globals maxb gl) mb id0 align0 F gn tsz
+  (Hal: malloc (los, nts) M tsz gn align0 = ret (M', mb)) 
+  (HwfM: wf_Mem maxb (los, nts) M)
+  (Hwflc : wf_lc M lc) (Hsize: getTypeAllocSize (los, nts) t = ret tsz),
    F = PI_f pinfo ->
-   inscope_of_pc F
-     (block_intro l1 ps1 (cs1' ++ insn_alloca id0 t v align0 :: cs) tmn)
-     (insn_alloca id0 t v align0 :: cs) tmn = ret ids0 ->
-   wf_defs maxb pinfo TD M lc ids0 als ->
-   wf_defs maxb pinfo TD M'
+   wf_defs maxb pinfo (los, nts) M lc als ->
+   wf_defs maxb pinfo (los, nts) M'
      (updateAddAL (GVsT DGVs) lc id0
-        ($ blk2GV TD mb # typ_pointer t $)) 
-     (id0 :: ids0) (mb :: als).
+        ($ blk2GV (los, nts) mb # typ_pointer t $)) (mb :: als).
 Proof.
   intros. unfold wf_defs. 
-  intros gvsa Hpindom Hlkp.
+  intros gvsa Hlkp.
   destruct (id_dec id0 (PI_id pinfo)); subst.
     rewrite lookupAL_updateAddAL_eq in Hlkp.
     inv Hlkp.
@@ -2122,7 +2387,7 @@ Proof.
           destruct HwfM. omega.
       split.
         intros.
-        assert (mload TD M gptr ty al = ret gvs1 \/
+        assert (mload (los, nts) M gptr ty al = ret gvs1 \/
                 forall v m, In (v, m) gvs1 -> v = Vundef) as J.
           eapply malloc_preserves_mload_inv; eauto.
         destruct J as [J | J].
@@ -2135,8 +2400,9 @@ Proof.
 
         rewrite simpl_blk2GV. 
         unfold mload. simpl.
-        assert (exists mc, flatten_typ TD (PI_typ pinfo) = Some mc) as J.
-          admit. (* wfPI *)
+        assert (exists mc, flatten_typ (los, nts) (PI_typ pinfo) = Some mc) 
+          as J.
+          eapply WF_PhiInfo_spec2; eauto.
         destruct J as [mc J].
         rewrite J.
         eapply mload_aux_malloc_same'; eauto.
@@ -2150,10 +2416,8 @@ Proof.
       apply malloc_result in Hal. subst. omega.
 
     rewrite <- lookupAL_updateAddAL_neq in Hlkp; auto.
-    simpl in Hpindom.
-    destruct Hpindom as [Hpindom | Hpindom]; subst; try congruence.
     assert (Hlkp':=Hlkp).
-    apply H1 in Hlkp; auto.
+    apply H0 in Hlkp; auto.
     destruct Hlkp as [J1 J2].
     split.
       destruct J1 as [[mb' [J31 [J32 J33]]] [J4 [gv J5]]]; subst.
@@ -2165,7 +2429,7 @@ Proof.
           omega.
       split.
         intros.
-        assert (mload TD M gptr ty al = ret gvs1 \/
+        assert (mload (los, nts) M gptr ty al = ret gvs1 \/
                 forall v m, In (v, m) gvs1 -> v = Vundef) as J.
           eapply malloc_preserves_mload_inv; eauto.
         destruct J as [J | J]; eauto.
@@ -2191,28 +2455,22 @@ Proof.
 Qed.
 
 Lemma malloc_preserves_wf_defs_at_head : forall maxb pinfo TD M  
-  M' gl als lc t v
-  (Hwfgl: wf_globals maxb gl) mb id0 tmn align0 cs cs1' l1 ps1 F gn tsz
+  M' gl als lc t 
+  (Hwfgl: wf_globals maxb gl) mb id0 align0 F gn tsz
   (Hal: malloc TD M tsz gn align0 = ret (M', mb)) (HwfM: wf_Mem maxb TD M)
-  (Hwflc : wf_lc M lc) (Hneq: id0 <> PI_id pinfo),
-  forall ids0,
+  (Hwflc : wf_lc M lc) (Hneq: F = PI_f pinfo -> id0 <> PI_id pinfo),
    F = PI_f pinfo ->
-   inscope_of_pc F
-     (block_intro l1 ps1 (cs1' ++ insn_malloc id0 t v align0 :: cs) tmn)
-     (insn_malloc id0 t v align0 :: cs) tmn = ret ids0 ->
-   wf_defs maxb pinfo TD M lc ids0 als ->
+   wf_defs maxb pinfo TD M lc als ->
    wf_defs maxb pinfo TD M'
      (updateAddAL (GVsT DGVs) lc id0
-        ($ blk2GV TD mb # typ_pointer t $)) 
-     (id0 :: ids0) als.
+        ($ blk2GV TD mb # typ_pointer t $)) als.
 Proof.
-  intros. unfold wf_defs. 
-  intros gvsa Hpindom Hlkp.
+  intros. unfold wf_defs.  
+  assert (JJ:=H). apply Hneq in JJ. subst.
+  intros gvsa Hlkp.
   rewrite <- lookupAL_updateAddAL_neq in Hlkp; auto.
-  simpl in Hpindom.
-  destruct Hpindom as [Hpindom | Hpindom]; subst; try congruence.
   assert (Hlkp':=Hlkp).
-  apply H1 in Hlkp; auto.
+  apply H0 in Hlkp; auto.
   destruct Hlkp as [J1 J2].
   split.
       destruct J1 as [[mb' [J31 [J32 J33]]] [J4 [gv J5]]]; subst.
@@ -2278,132 +2536,68 @@ Ltac simpl_ctx Hinv HwfS1 :=
   fold (@OpsemPP.wf_ECStack DGVs) in HwfEC0;
   destruct HwfS1 as [[HwfEC [HwfECs Hwfht]] [Hnonup1 HwfM1]].
 
-Lemma preservation : forall maxb pinfo cfg S1 S2 tr
-  (Hinv: OpsemPP.wf_State cfg S1)
-  (Hwfg: wf_globals maxb (OpsemAux.Globals cfg)) (Hinbd: 0 <= maxb)
-  (HwfPI: WF_PhiInfo pinfo) (HsInsn: Opsem.sInsn cfg S1 S2 tr)
-  (HwfS1: wf_State maxb pinfo cfg S1), wf_State maxb pinfo cfg S2.
+Ltac preservation_tac4 :=
+  match goal with
+  | HwfPI : WF_PhiInfo _,
+    HFinPs1: InProductsB _ _ = _,
+    HBinF1: blockInFdefB _ _ = _,
+    HmInS: moduleInSystemB _ _ = _,
+    HwfSystem: wf_system _ _ |- _ =>
+    simpl; intros; subst;
+    clear - HBinF1 HFinPs1 HmInS HwfPI HwfSystem;
+    eapply wf_system__uniqFdef in HFinPs1; eauto;
+    eapply IngetCmdsIDs__lookupCmdViaIDFromFdef in HBinF1; 
+      eauto using in_middle;
+    eapply WF_PhiInfo_spec3 in HBinF1; eauto; simpl; auto;
+    simpl in HBinF1;
+    apply orb_false_iff in HBinF1; destruct HBinF1; auto
+  end.
+
+Lemma preservation_Call: forall (maxb : Z) (pinfo : PhiInfo)
+  (F : fdef) (B : block) (lc : Opsem.GVsMap) (rid : id) (noret0 : noret)
+  (ca : clattrs) (fv : value) (lp : params) (cs : list cmd) (tmn : terminator)
+  (EC : list Opsem.ExecutionContext) (Mem : mem) (als : list mblock) (ft : typ)
+  ECs cfg S los nts Ps gl fs
+  (EQ1 : cfg = OpsemAux.mkCfg S (los, nts) Ps gl fs)
+  (EQ2 : ECs = {| Opsem.CurFunction := F;
+                 Opsem.CurBB := B;
+                 Opsem.CurCmds := insn_call rid noret0 ca ft fv lp :: cs;
+                 Opsem.Terminator := tmn;
+                 Opsem.Locals := lc;
+                 Opsem.Allocas := als |} :: EC)
+  (Hinv : OpsemPP.wf_State cfg        
+           {| Opsem.ECS := ECs;
+              Opsem.Mem := Mem |})
+  (Hwfg : wf_globals maxb gl)
+  (Hinbd : 0 <= maxb) (HwfPI : WF_PhiInfo pinfo) (fid : id) (fptrs : GVsT DGVs)
+  (fptr : GenericValue) (lc' : Opsem.GVsMap) (l' : l) (ps' : phinodes)
+  (cs' : cmds) (tmn' : terminator) (rt : typ) (la : args) (va : varg)
+  (lb : blocks) (fa : fnattrs) (gvs : list (GVsT DGVs))
+  (H : Opsem.getOperandValue (los, nts) fv lc gl = ret fptrs)
+  (H0 : fptr @ fptrs)
+  (H1 : OpsemAux.lookupFdefViaPtr Ps fs fptr =
+        ret fdef_intro (fheader_intro fa rt fid la va) lb)
+  (H2 : getEntryBlock (fdef_intro (fheader_intro fa rt fid la va) lb) =
+        ret block_intro l' ps' cs' tmn')
+  (H3 : Opsem.params2GVs (los, nts) lp lc gl = ret gvs)
+  (H4 : Opsem.initLocals (los, nts) la gvs = ret lc')
+  (HwfS1 : wf_State maxb pinfo cfg
+            {| Opsem.ECS := ECs;
+               Opsem.Mem := Mem |}),
+  wf_State maxb pinfo cfg
+     {|
+     Opsem.ECS := {|
+                  Opsem.CurFunction := fdef_intro
+                                         (fheader_intro fa rt fid la va) lb;
+                  Opsem.CurBB := block_intro l' ps' cs' tmn';
+                  Opsem.CurCmds := cs';
+                  Opsem.Terminator := tmn';
+                  Opsem.Locals := lc';
+                  Opsem.Allocas := nil |}
+                  :: ECs;
+     Opsem.Mem := Mem |}.
 Proof.
-  intros.
-  (sInsn_cases (induction HsInsn) Case); destruct TD as [los nts]; simpl HwfS1.
-
-Case "sReturn". eapply preservation_return; eauto. 
-Case "sReturnVoid". admit.
-Case "sBranch". admit.
-Case "sBranch_uncond". admit.
-Case "sBop".
-  eapply preservation_pure_cmd_updated_case in HwfS1; try solve [simpl; eauto]; 
-    eauto.
-    eapply BOP__wf_GVs_in_ECs; eauto.
-      admit. (* WF *)
-Case "sFBop". admit.
-Case "sExtractValue". admit. 
-(* tricky case, 
-   we need to ensure that all extractable values cannot be aliased *)
-Case "sInsertValue". admit. 
-(* tricky case, 
-   we need to ensure that we are not inserting aliased values *)
-Case "sMalloc". 
-  simpl_ctx Hinv HwfS1.
-  split.
-    split.
-      eapply impure_cmd_updated_preserves_wf_EC; eauto.
-        intros. subst.
-        apply wf_EC__wf_lc in HwfEC.
-        eapply malloc_preserves_wf_defs_at_head with (tmn:=tmn); eauto.
-          admit. (* WF PI *)
-        eapply malloc_preserves_wf_lc; eauto.
-    split.
-      eapply malloc_preserves_wf_ECStack_in_tail in H2; eauto.
-      eapply malloc_preserves_wf_ECStack_head_tail in H2; eauto.
-  split.
-    destruct HwfM1.
-    eapply malloc_preserves_wf_als in H2; eauto.
-      simpl_env in H2.
-      apply wf_als_split in H2. destruct H2; auto.
-    eapply malloc_preserves_wf_Mem in H2; eauto.
-
-Case "sFree". 
-  simpl_ctx Hinv HwfS1.
-  split.
-    split.
-      eapply impure_cmd_non_updated_preserves_wf_EC with (M:=Mem); eauto.
-        intros. subst.
-        eapply free_preserves_wf_defs_at_head; eauto.
-          admit. (* WF PhiInfo *)
-        eapply free_preserves_wf_lc; eauto.
-    split.
-      eapply free_preserves_wf_ECStack_in_tail in H1; eauto.
-      eapply free_preserves_wf_ECStack_head_tail in H1; eauto.
-  split.
-    eapply free_preserves_wf_als in H1; eauto.
-    eapply free_preserves_wf_Mem in H1; eauto.
-
-Case "sAlloca". 
-  simpl_ctx Hinv HwfS1.
-  split.
-    split.
-      eapply impure_cmd_updated_preserves_wf_EC; eauto.
-        intros. subst.
-        apply wf_EC__wf_lc in HwfEC.
-        eapply alloca_preserves_wf_defs_at_head; eauto.
-        eapply malloc_preserves_wf_lc; eauto.
-    split.       
-      eapply malloc_preserves_wf_ECStack_in_tail in H2; eauto.
-      eapply malloc_preserves_wf_ECStack_head_tail in H2; eauto.
-  split.
-    destruct HwfM1.
-    eapply malloc_preserves_wf_als in H2; eauto.
-    eapply malloc_preserves_wf_Mem in H2; eauto.
-
-Case "sLoad". 
-  eapply preservation_pure_cmd_updated_case in HwfS1; try solve [simpl; eauto]; 
-    eauto.
-    destruct HwfS1 as [[[_ Hwflc] [_ Hwfstk]] [_ HwfM]]. 
-    eapply mload__wf_GVs_in_ECs; eauto using wf_EC__wf_lc.
-      admit. (* WF *)
-Case "sStore". 
-  simpl_ctx Hinv HwfS1.
-  assert (wf_lc Mem lc) as Hwflc.
-    apply wf_EC__wf_lc in HwfEC; auto.
-  split.
-    split.
-      eapply impure_cmd_non_updated_preserves_wf_EC with (M:=Mem); eauto.
-        intros. subst.
-        eapply mstore_preserves_wf_defs_at_head with (gvs1:=gvs1) in H3; eauto.
-          admit. (* WF PhiInfo *)
-        eapply mstore_preserves_wf_lc; eauto.
-    split.
-      eapply mstore_preserves_wf_ECStack_in_tail with (gvs1:=gvs1) in H3; eauto.
-      eapply mstore_preserves_wf_ECStack_head_tail' with (gvs1:=gvs1) in H3; 
-        eauto.
-  split.
-    eapply mstore_preserves_wf_als in H3; eauto.
-    eapply mstore_preserves_wf_Mem with (gvs1:=gvs1) in H3; eauto.
-
-Case "sGEP". 
-  eapply preservation_pure_cmd_updated_case in HwfS1; try solve [simpl; eauto]; 
-    eauto.
-    destruct HwfS1 as [[[_ Hwflc] [_ Hwfstk]] [_ [_ HwfM]]]. 
-    eapply GEP__wf_GVs_in_ECs; eauto using wf_EC__wf_lc.
-      admit. (* WF PI *)
-      admit. (* WF *)
-
-Case "sTrunc". admit.
-Case "sExt". admit.
-Case "sCast". 
-  eapply preservation_pure_cmd_updated_case in HwfS1; try solve [simpl; eauto]; 
-    eauto.
-    destruct HwfS1 as [[[_ Hwflc] [_ Hwfstk]] [_ [_ HwfM]]]. 
-    eapply CAST__wf_GVs_in_ECs; eauto.
-      admit. (* WF PI *)
-      admit. (* WF *)
-
-Case "sIcmp". admit.
-Case "sFcmp". admit.
-Case "sSelect". admit. (* can return ptr *)
-Case "sCall". 
-Focus.
+  intros. subst.
   destruct Hinv as 
     [_ [HwfSystem [HmInS [Hnonempty [
      [Hreach1 [HBinF1 [HFinPs1 [_ [_ [l1 [ps1 [cs1' Heq1]]]]]]]] 
@@ -2434,33 +2628,1038 @@ Focus.
         eapply entryBlock_has_no_phinodes with (ifs:=nil)(s:=S); eauto.        
       subst.
       apply dom_entrypoint in H2. 
-      unfold inscope_of_pc in *.
-      destruct cs'.
-        unfold inscope_of_tmn.
-        remember ((dom_analyze (fdef_intro (fheader_intro fa rt fid la va) lb)) 
-          !! l') as R.
-        destruct R. simpl in H2. subst. simpl.
-
-        eapply initLocals_preserves_wf_defs; eauto.
-
-        unfold inscope_of_cmd, inscope_of_id.
-        remember ((dom_analyze (fdef_intro (fheader_intro fa rt fid la va) lb)) 
-          !! l') as R.
-        destruct R. simpl. simpl in H2. subst. simpl.
-        destruct (eq_atom_dec (getCmdLoc c) (getCmdLoc c)) as [|n]; 
-          try solve [contradict n; auto]. 
-        eapply initLocals_preserves_wf_defs; eauto.
+      eapply initLocals_preserves_wf_defs; eauto.
 
       destruct HwfM.
       eapply initLocals_preserves_wf_lc; eauto.
 
   split.
     repeat (split; auto). 
-    simpl.
+    assert(PI_f pinfo = F -> 
+           fold_left
+             (fun (acc : bool) (p : typ * attributes * value) =>
+              let '(_, v) := p in used_in_value (PI_id pinfo) v || acc) lp false
+              = false) as J.
+      preservation_tac4.
     eapply initLocals_preserves_wf_ECStack_head_tail; eauto.
-      simpl. admit. (* WFPI *)
+Qed.
 
-Unfocus.
+Lemma preservation_return_void : forall maxb pinfo (HwfPI : WF_PhiInfo pinfo)  
+  F B rid lc F' B' c' cs' tmn' lc' EC Mem als als' cfg
+  EC1 EC2 (Hwfg: wf_globals maxb (OpsemAux.Globals cfg))
+  (EQ1:EC1 = {| Opsem.CurFunction := F;
+                Opsem.CurBB := B;
+                Opsem.CurCmds := nil;
+                Opsem.Terminator := insn_return_void rid;
+                Opsem.Locals := lc;
+                Opsem.Allocas := als |})
+  (EQ2:EC2 = {| Opsem.CurFunction := F';
+                Opsem.CurBB := B';
+                Opsem.CurCmds := c' :: cs';
+                Opsem.Terminator := tmn';
+                Opsem.Locals := lc';
+                Opsem.Allocas := als' |})
+  (Hinv : OpsemPP.wf_State cfg
+           {| Opsem.ECS := EC1 :: EC2 :: EC;
+              Opsem.Mem := Mem |})
+  Mem' (H : Instruction.isCallInst c' = true)
+  (H0 : free_allocas (OpsemAux.CurTargetData cfg) Mem als = ret Mem')
+  (H1 : getCallerReturnID c' = merror)
+  (HwfS1 : wf_State maxb pinfo cfg
+            {| Opsem.ECS := EC1 :: EC2 :: EC;
+               Opsem.Mem := Mem |}),
+  wf_State maxb pinfo cfg
+     {| Opsem.ECS :=
+             {| Opsem.CurFunction := F';
+                Opsem.CurBB := B';
+                Opsem.CurCmds := cs';
+                Opsem.Terminator := tmn';
+                Opsem.Locals := lc';
+                Opsem.Allocas := als' |} :: EC;
+        Opsem.Mem := Mem' |}.
+Proof.
+Local Opaque inscope_of_tmn inscope_of_cmd.
+
+  intros. subst. destruct cfg as [S [los nts] Ps gl fs]. 
+  destruct Hinv as 
+    [_ [HwfSystem [HmInS [Hnonempty [
+     [Hreach1 [HBinF1 [HFinPs1 [_ [_ [l1 [ps1 [cs1' Heq1]]]]]]]] 
+     [
+       [
+         [Hreach2 [HBinF2 [HFinPs2 [_ [_ [l2 [ps2 [cs2' Heq2]]]]]]]]
+         [HwfEC0 HwfCall]
+       ]
+       HwfCall'
+     ]
+    ]]]]]; subst.
+  fold (@OpsemPP.wf_ECStack DGVs) in HwfEC0.
+  destruct HwfS1 as 
+    [
+      [[Hinscope1 Hwflc1] [[[Hinscope2 Hwflc2] [HwfECs Hfr2]] Hfr1]] 
+      [Hdisjals HwfM]
+    ]. simpl. simpl in Hdisjals.
+  fold wf_ECStack in HwfECs.
+  assert (Hdisjals':=Hdisjals).
+  destruct Hdisjals' as [Hdisjals' _].
+  split.
+  SCase "wf_ECStack".
+    split.
+    SSCase "wf_EC".
+    split.
+    SSSCase "sdom".
+      destruct (fdef_dec (PI_f pinfo) F'); subst; auto.
+      remember (getCmdID c') as R.
+      destruct c'; try solve [inversion H].
+      assert (In (insn_call i0 n c t v p) 
+        (cs2'++[insn_call i0 n c t v p] ++ cs')) as HinCs.
+        apply in_or_app. right. simpl. auto.
+      assert (Hwfc := HBinF2).
+      eapply wf_system__wf_cmd with (c:=insn_call i0 n c t v p) in Hwfc; eauto.
+      assert (wf_fdef nil S (module_intro los nts Ps) (PI_f pinfo)) as HwfF.
+        eapply wf_system__wf_fdef; eauto.
+      assert (uniqFdef (PI_f pinfo)) as HuniqF.
+        eapply wf_system__uniqFdef; eauto.
+      
+      assert (NoDup (als ++ als')) as Hnodup.
+        rewrite_env 
+          ((als ++ als') ++ 
+            flat_map
+              (fun ec : Opsem.ExecutionContext =>
+               let '{| Opsem.Allocas := als |} := ec in als) EC) in Hdisjals'.
+        apply NoDup_split in Hdisjals'.
+        destruct Hdisjals'; auto.
+      eapply free_allocas_preserves_wf_defs in Hinscope2; eauto.
+
+    SSSCase "wflc".
+      clear - Hwflc1 Hwflc2 H1 Hwfg HwfM H0.
+      eapply free_allocas_preserves_wf_lc in H0; eauto.
+
+    split.
+    SSCase "wf_ECs".
+      eapply free_allocas_preserves_wf_ECStack; eauto.
+      apply NoDup_strenthening in Hdisjals'; auto.
+
+    SSCase "wf_ECs_head_tail".
+      simpl in Hfr1, Hfr2.
+      eapply free_allocas_preserves_wf_ECStack_head_tail'; eauto.
+
+  split.
+  SCase "Disjoint Allocas".
+    apply wf_als_split in Hdisjals.
+    destruct Hdisjals; auto.
+    eapply free_allocas_preserves_wf_als; eauto.
+
+  SCase "wfM".
+    eapply free_allocas_preserves_wf_Mem; eauto.
+
+Transparent inscope_of_tmn inscope_of_cmd.
+Qed.
+
+
+Lemma getIncomingValuesForBlockFromPHINodes_spec9: forall TD gl lc b id0 gvs0
+  ps' l0,
+  ret l0 = Opsem.getIncomingValuesForBlockFromPHINodes TD ps' b gl lc ->
+  id0 `in` dom l0 ->
+  lookupAL (GVsT DGVs) l0 id0 = ret gvs0 ->
+  exists id1, exists t1, exists vls1, exists v, exists n,
+    In (insn_phi id1 t1 vls1) ps' /\
+    nth_list_value_l n vls1 = Some (v, getBlockLabel b) /\
+    Opsem.getOperandValue TD v lc gl= Some gvs0.
+Proof.
+  induction ps' as [|[]]; simpl; intros.
+    inv H. fsetdec.
+    
+    inv_mbind'. simpl in *.
+    destruct (id0 == i0); subst.
+      inv H1.
+      destruct b. simpl in *.
+      symmetry in HeqR.
+      apply getValueViaLabelFromValuels__nth_list_value_l in HeqR; auto.
+      destruct HeqR as [n HeqR].
+      exists i0. exists t. exists l0. exists v. exists n.
+      split; auto.
+
+      apply IHps' in H1; auto; try fsetdec.
+      destruct H1 as [id1 [t1 [vls1 [v' [n' [J1 [J2 J3]]]]]]].
+      exists id1. exists t1. exists vls1. exists v'. exists n'.
+      split; auto.
+Qed.
+
+Lemma IngetPhiNodesIDs__lookupPhiNodeViaIDFromPhiNodes: forall id2 ps1
+  (H0 : In id2 (getPhiNodesIDs ps1)),
+  exists p2, lookupPhiNodeViaIDFromPhiNodes ps1 id2 = Some p2 /\
+             getPhiNodeID p2 = id2.
+Proof.
+  induction ps1; simpl; intros.
+    inv H0.
+
+    destruct H0 as [H0 | H0]; subst.
+      destruct (getPhiNodeID a == getPhiNodeID a); eauto.
+        congruence.
+
+      destruct (@eq_dec id (EqDec_eq_of_EqDec id EqDec_atom) (getPhiNodeID a) 
+                 id2); subst; eauto.
+Qed.
+
+Lemma lookupInsnViaIDFromBlocks__In : forall id0 instr bs,
+  lookupInsnViaIDFromBlocks bs id0 = Some instr ->
+  In id0 (getBlocksLocs bs).
+Proof.
+  induction bs; simpl; intros.
+    inv H.
+
+    apply in_or_app.
+    remember (lookupInsnViaIDFromBlock a id0) as R.
+    destruct R; eauto.
+      inv H.
+      symmetry in HeqR.
+      apply lookupInsnViaIDFromBlock__In in HeqR; auto.
+Qed.
+
+Lemma IngetPhiNodesIDs__lookupPhinodeViaIDFromFdef: forall id2 l1 ps1 cs1 tmn1 f
+  (Huniq: uniqFdef f)
+  (H : blockInFdefB (block_intro l1 ps1 cs1 tmn1) f = true)
+  (H0 : In id2 (getPhiNodesIDs ps1)),
+  exists p2, lookupInsnViaIDFromFdef f id2 = Some (insn_phinode p2) /\
+             getPhiNodeID p2 = id2.
+Proof.
+  destruct f as [[] bs]. simpl. intros.
+  destruct Huniq as [_ Huniq].
+  apply NoDup_split in Huniq.
+  destruct Huniq as [_ Huniq].
+  generalize dependent l1.
+  generalize dependent ps1.
+  generalize dependent cs1.
+  generalize dependent tmn1.
+  generalize dependent id2.
+  induction bs; simpl; intros.
+    congruence.
+
+    apply orb_true_iff in H.
+    destruct H as [H | H].
+      apply blockEqB_inv in H.
+      subst. simpl.
+      apply IngetPhiNodesIDs__lookupPhiNodeViaIDFromPhiNodes in H0.
+      destruct H0 as [ps [H0 Heq]]; subst.
+      rewrite H0. eauto.
+
+      simpl_env in Huniq. rewrite getBlocksLocs_app in Huniq.
+      assert (Huniq':=Huniq).
+      apply NoDup_inv in Huniq'. destruct Huniq'.
+      eapply IHbs in H; eauto.
+      destruct H as [p2 [H Heq]]; subst.
+      rewrite H. 
+      apply lookupInsnViaIDFromBlocks__In in H.
+      eapply infrastructure_props.NoDup_disjoint in Huniq; eauto.
+      simpl in Huniq. simpl_env in Huniq.
+      apply notin__lookupInsnViaIDFromBlock_none in Huniq.
+      rewrite Huniq. eauto.
+Qed.
+
+Lemma unused_in_phi__wf_use_at_head: forall pinfo id1 t1 vls1 ps' v1 l1 n,
+  used_in_phi (PI_id pinfo) (insn_phi id1 t1 vls1) = false ->
+  In (insn_phi id1 t1 vls1) ps' ->
+  nth_list_value_l n vls1 = ret (v1, l1) ->
+  wf_use_at_head pinfo v1.      
+Admitted.
+
+Lemma In_InPhiNodesB: forall p ps, In p ps -> InPhiNodesB p ps.
+Proof.
+  induction ps; simpl; intros.
+    inv H.
+    apply orb_true_iff.
+    destruct H as [H | H]; subst.
+      left. apply phinodeEqB_refl.
+      right. apply IHps; auto.
+Qed.
+
+Lemma wf_defs_br : forall lc l' ps' cs' lc' tmn' gl los nts Ps ifs s
+  (l3 : l) (ps : phinodes) (cs : list cmd) tmn pinfo (Hwfpi: WF_PhiInfo pinfo)
+  (Hlkup : Some (block_intro l' ps' cs' tmn') = 
+             lookupBlockViaLabelFromFdef (PI_f pinfo) l')
+  (Hswitch : Opsem.switchToNewBasicBlock (los,nts) (block_intro l' ps' cs' tmn')
+         (block_intro l3 ps cs tmn) gl lc = ret lc')
+  als Mem maxb 
+  (Hwfdfs : wf_defs maxb pinfo (los,nts) Mem lc als)
+  (Hwflc : wf_lc Mem lc)
+  (Hwfg : wf_globals maxb gl)
+  (HwfF : wf_fdef ifs s (module_intro los nts Ps) (PI_f pinfo))
+  (Huniq : uniqFdef (PI_f pinfo)),
+  wf_defs maxb pinfo (los,nts) Mem lc' als.
+Proof.
+  intros.
+  unfold Opsem.switchToNewBasicBlock in Hswitch. simpl in Hswitch.
+  inv_mbind'.
+  intros gvsa Hlkup'.
+  assert (lookupAL (GVsT DGVs) lc (PI_id pinfo) = ret gvsa) as Hlkp.
+    destruct (@AtomSetProperties.In_dec (PI_id pinfo) (dom l0)) 
+      as [Hin | Hnotin].
+      eapply OpsemProps.getIncomingValuesForBlockFromPHINodes_spec7 in Hin; 
+        eauto.
+      contradict Hin.
+      eapply WF_PhiInfo_spec6 in Hlkup; eauto. 
+      
+      apply OpsemProps.updateValuesForNewBlock_spec7 in Hlkup'; auto.
+  assert (J3:=Hlkp).
+  apply Hwfdfs in J3.
+  destruct J3 as [J1 J2].
+  split; auto.
+    intros.
+    destruct (@AtomSetProperties.In_dec id0 (dom l0)) as [Hin | Hnotin].
+      rewrite OpsemProps.updateValuesForNewBlock_spec6' in Hlk0; auto.
+      eapply getIncomingValuesForBlockFromPHINodes_spec9 in HeqR; eauto.
+      destruct HeqR as [id1 [t1 [vls1 [v [n [J4 [J5 J6]]]]]]].
+      unfold wf_non_alloca_GVs.
+      destruct (id_dec id0 (PI_id pinfo)); auto.
+      eapply operand__no_alias_with__head; eauto.
+        symmetry in Hlkup.
+        apply lookupBlockViaLabelFromFdef_inv in Hlkup; auto.
+        destruct Hlkup as [_ Hlkup].
+        assert (phinodeInFdefBlockB (insn_phi id1 t1 vls1) (PI_f pinfo) 
+          (block_intro l' ps' cs' tmn') = true) as Hin'.
+          apply andb_true_iff.
+          split; auto.
+          simpl.
+          apply In_InPhiNodesB; auto.
+        apply WF_PhiInfo_spec5 in Hin'; auto.
+        eapply unused_in_phi__wf_use_at_head in Hin'; eauto.
+
+      apply OpsemProps.updateValuesForNewBlock_spec7 in Hlk0; auto.
+Qed.
+
+Lemma wf_lc_br : forall (lc:DGVMap) l' ps' cs' lc' tmn' gl td 
+  (l3 : l) (ps : phinodes) (cs : list cmd) tmn F
+  (Hlkup : Some (block_intro l' ps' cs' tmn') = 
+             lookupBlockViaLabelFromFdef F l')
+  (Hswitch : Opsem.switchToNewBasicBlock td (block_intro l' ps' cs' tmn')
+         (block_intro l3 ps cs tmn) gl lc = ret lc')
+  Mem maxb (Hwflc : wf_lc Mem lc) (HwfM : wf_Mem maxb td Mem)
+  (Hwfg : wf_globals maxb gl)
+  (Huniq : uniqFdef F),
+  wf_lc Mem lc'.
+Proof.
+  intros.
+  unfold Opsem.switchToNewBasicBlock in Hswitch. simpl in Hswitch.
+  inv_mbind'.
+  intros id0 gvs0 Hlkup'.
+  destruct (@AtomSetProperties.In_dec id0 (dom l0)) as [Hin | Hnotin].
+      rewrite (@OpsemProps.updateValuesForNewBlock_spec6' DGVs) in Hlkup'; auto.
+      eapply getIncomingValuesForBlockFromPHINodes_spec9 in HeqR; eauto.
+      destruct HeqR as [id1 [t1 [vls1 [v [n [J4 [J5 J6]]]]]]].
+      destruct HwfM.
+      eapply operand__lt_nextblock; eauto.
+
+      apply (@OpsemProps.updateValuesForNewBlock_spec7 DGVs) in Hlkup'; auto.
+      apply Hwflc in Hlkup'; auto.
+Qed.
+
+Lemma wf_ECStack_head_tail_br : forall (lc:DGVMap) l' ps' cs' lc' tmn' gl los 
+  nts Ps ifs s (l3 : l) (ps : phinodes) (cs : list cmd) tmn F
+  (Hlkup : Some (block_intro l' ps' cs' tmn') = 
+             lookupBlockViaLabelFromFdef F l')
+  (Hswitch : Opsem.switchToNewBasicBlock (los,nts) (block_intro l' ps' cs' tmn')
+         (block_intro l3 ps cs tmn) gl lc = ret lc') EC pinfo
+  Mem maxb (Hwflc : wf_ECStack_head_tail maxb pinfo (los, nts) Mem lc EC) 
+  (HwfM : wf_Mem maxb (los, nts) Mem)
+  (Hwfg : wf_globals maxb gl)
+  (HwfF : wf_fdef ifs s (module_intro los nts Ps) F)
+  (Huniq : uniqFdef F),
+  wf_ECStack_head_tail maxb pinfo (los, nts) Mem lc' EC.
+Proof.
+  intros.
+  unfold Opsem.switchToNewBasicBlock in Hswitch. simpl in Hswitch.
+  inv_mbind'.
+  intros ec0 Hintl.
+  apply Hwflc in Hintl.
+  destruct ec0. simpl in *.
+  intros. subst.
+  assert (H0':=H0).
+  apply Hintl in H0; auto.
+  destruct H0 as [J1 [J2 J3]].
+  split; auto.
+  split; auto.
+    intros.
+    destruct (@AtomSetProperties.In_dec id1 (dom l0)) as [Hin | Hnotin].
+      rewrite (@OpsemProps.updateValuesForNewBlock_spec6' DGVs) in H; auto.
+      eapply getIncomingValuesForBlockFromPHINodes_spec9 in HeqR; eauto.
+      destruct HeqR as [id2 [t1 [vls1 [v [n [J4 [J5 J6]]]]]]].
+      eapply operand__no_alias_with__tail with
+        (EC:={|
+            Opsem.CurFunction := PI_f pinfo;
+            Opsem.CurBB := CurBB;
+            Opsem.CurCmds := CurCmds;
+            Opsem.Terminator := Terminator;
+            Opsem.Locals := Locals;
+            Opsem.Allocas := Allocas |}); eauto; simpl; auto.
+
+      apply (@OpsemProps.updateValuesForNewBlock_spec7 DGVs) in H; eauto.
+Qed.
+
+Lemma preservation_branch: forall (maxb : Z) (pinfo : PhiInfo) (S : system)
+  (los : layouts) (nts : namedts) (Ps : list product) (F : fdef) (B : block)
+  (lc : Opsem.GVsMap) (gl : GVMap) (fs : GVMap) (bid : id) (Cond : value)
+  (l1 : l) (l2 : l) (EC : list Opsem.ExecutionContext) (Mem : mem) 
+  (als : list mblock) cfg ECs
+  (EQ1 : cfg = OpsemAux.mkCfg S (los, nts) Ps gl fs)
+  (EQ2 : ECs = {| Opsem.CurFunction := F;
+                 Opsem.CurBB := B;
+                 Opsem.CurCmds := nil;
+                 Opsem.Terminator := insn_br bid Cond l1 l2;
+                 Opsem.Locals := lc;
+                 Opsem.Allocas := als |} :: EC)
+  (Hinv : OpsemPP.wf_State cfg
+           {| Opsem.ECS := ECs; Opsem.Mem := Mem |})
+  (Hwfg : wf_globals maxb
+           (OpsemAux.Globals
+              {|
+              OpsemAux.CurSystem := S;
+              OpsemAux.CurTargetData := (los, nts);
+              OpsemAux.CurProducts := Ps;
+              OpsemAux.Globals := gl;
+              OpsemAux.FunTable := fs |}))
+  (Hinbd : 0 <= maxb) (HwfPI : WF_PhiInfo pinfo) (conds : GVsT DGVs)
+  (c : GenericValue) (l' : l) (ps' : phinodes) (cs' : cmds) (tmn' : terminator)
+  (lc' : Opsem.GVsMap)
+  (H : Opsem.getOperandValue (los, nts) Cond lc gl = ret conds)
+  (H0 : c @ conds)
+  (H1 : ret block_intro l' ps' cs' tmn' =
+       (if isGVZero (los, nts) c
+        then lookupBlockViaLabelFromFdef F l2
+        else lookupBlockViaLabelFromFdef F l1))
+  (H2 : Opsem.switchToNewBasicBlock (los, nts) (block_intro l' ps' cs' tmn') B
+         gl lc = ret lc')
+  (HwfS1 : wf_State maxb pinfo cfg
+            {| Opsem.ECS := ECs; Opsem.Mem := Mem |}),
+  wf_State maxb pinfo cfg
+     {|
+     Opsem.ECS := {|
+                  Opsem.CurFunction := F;
+                  Opsem.CurBB := block_intro l' ps' cs' tmn';
+                  Opsem.CurCmds := cs';
+                  Opsem.Terminator := tmn';
+                  Opsem.Locals := lc';
+                  Opsem.Allocas := als |} :: EC;
+     Opsem.Mem := Mem |}.
+Proof.
+  intros. subst.
+  destruct Hinv as 
+    [_ [HwfSystem [HmInS [Hnonempty [
+     [Hreach1 [HBinF1 [HFinPs1 [_ [_ [l3 [ps3 [cs3' Heq1]]]]]]]] 
+     [HwfEC HwfCall]
+     ]
+    ]]]]; subst.
+  fold (@OpsemPP.wf_ECStack DGVs) in HwfEC.
+  destruct HwfS1 as [[[Hinscope1 Hwflc1] [HwfECs Hfr1]] [Hdisjals HwfM]]. 
+  simpl. simpl in Hdisjals.
+  fold wf_ECStack in HwfECs.
+  assert (Hdisjals':=Hdisjals).
+  destruct Hdisjals' as [Hdisjals' _].
+  assert (HwfF := HwfSystem).
+  eapply wf_system__wf_fdef with (f:=F) in HwfF; eauto.
+  assert (HuniqF := HwfSystem).
+  eapply wf_system__uniqFdef with (f:=F) in HuniqF; eauto.
+  assert (ret block_intro l' ps' cs' tmn' =
+    lookupBlockViaLabelFromFdef F l') as Hlkup.
+    symmetry.
+    apply blockInFdefB_lookupBlockViaLabelFromFdef; auto.
+    symmetry in H1.
+    destruct (isGVZero (los, nts) c);
+      apply lookupBlockViaLabelFromFdef_inv in H1; 
+        try solve [auto | destruct H1; auto].
+  split; auto.
+  split.
+  SCase "wf_ECStack".
+    split.
+      SSCase "sdom".
+      destruct (fdef_dec (PI_f pinfo) F); subst; auto.
+        eapply wf_defs_br; eauto.
+      SSCase "wf_lc".
+      eapply wf_lc_br; eauto.
+  split; auto.
+  SCase "wf_ECs_tail".
+    eapply wf_ECStack_head_tail_br; eauto.
+Qed.
+
+Lemma preservation_branch_uncond: forall (maxb : Z) (pinfo : PhiInfo) 
+  (S : system) (los : layouts) (nts : namedts) (Ps : list product) (F : fdef) 
+  (B : block) (lc : Opsem.GVsMap) (gl : GVMap) (fs : GVMap) (bid : id) 
+  (l0 : l) (EC : list Opsem.ExecutionContext) (Mem : mem) 
+  (als : list mblock) cfg ECs
+  (EQ1 : cfg = OpsemAux.mkCfg S (los, nts) Ps gl fs)
+  (EQ2 : ECs = {| Opsem.CurFunction := F;
+                 Opsem.CurBB := B;
+                 Opsem.CurCmds := nil;
+                 Opsem.Terminator := insn_br_uncond bid l0;
+                 Opsem.Locals := lc;
+                 Opsem.Allocas := als |} :: EC)
+  (Hinv : OpsemPP.wf_State cfg
+           {| Opsem.ECS := ECs; Opsem.Mem := Mem |})
+  (Hwfg : wf_globals maxb
+           (OpsemAux.Globals
+              {|
+              OpsemAux.CurSystem := S;
+              OpsemAux.CurTargetData := (los, nts);
+              OpsemAux.CurProducts := Ps;
+              OpsemAux.Globals := gl;
+              OpsemAux.FunTable := fs |}))
+  (Hinbd : 0 <= maxb) (HwfPI : WF_PhiInfo pinfo)
+  (l' : l) (ps' : phinodes) (cs' : cmds) (tmn' : terminator)
+  (lc' : Opsem.GVsMap)
+  (H1 : ret block_intro l' ps' cs' tmn' = lookupBlockViaLabelFromFdef F l0)
+  (H2 : Opsem.switchToNewBasicBlock (los, nts) (block_intro l' ps' cs' tmn') B
+         gl lc = ret lc')
+  (HwfS1 : wf_State maxb pinfo cfg
+            {| Opsem.ECS := ECs; Opsem.Mem := Mem |}),
+  wf_State maxb pinfo cfg
+     {|
+     Opsem.ECS := {|
+                  Opsem.CurFunction := F;
+                  Opsem.CurBB := block_intro l' ps' cs' tmn';
+                  Opsem.CurCmds := cs';
+                  Opsem.Terminator := tmn';
+                  Opsem.Locals := lc';
+                  Opsem.Allocas := als |} :: EC;
+     Opsem.Mem := Mem |}.
+Proof.
+  intros. subst.
+  destruct Hinv as 
+    [_ [HwfSystem [HmInS [Hnonempty [
+     [Hreach1 [HBinF1 [HFinPs1 [_ [_ [l3 [ps3 [cs3' Heq1]]]]]]]] 
+     [HwfEC HwfCall]
+     ]
+    ]]]]; subst.
+  fold (@OpsemPP.wf_ECStack DGVs) in HwfEC.
+  destruct HwfS1 as [[[Hinscope1 Hwflc1] [HwfECs Hfr1]] [Hdisjals HwfM]]. 
+  simpl. simpl in Hdisjals.
+  fold wf_ECStack in HwfECs.
+  assert (Hdisjals':=Hdisjals).
+  destruct Hdisjals' as [Hdisjals' _].
+  assert (HwfF := HwfSystem).
+  eapply wf_system__wf_fdef with (f:=F) in HwfF; eauto.
+  assert (HuniqF := HwfSystem).
+  eapply wf_system__uniqFdef with (f:=F) in HuniqF; eauto.
+  assert (ret block_intro l' ps' cs' tmn' = lookupBlockViaLabelFromFdef F l') 
+    as Hlkup.
+    symmetry.
+    apply blockInFdefB_lookupBlockViaLabelFromFdef; auto.
+    symmetry in H1.
+    apply lookupBlockViaLabelFromFdef_inv in H1; 
+        try solve [auto | destruct H1; auto].
+  split; auto.
+  split.
+  SCase "wf_ECStack".
+    split.
+      SSCase "sdom".
+      destruct (fdef_dec (PI_f pinfo) F); subst; auto.
+        eapply wf_defs_br; eauto.
+      SSCase "wf_lc".
+      eapply wf_lc_br; eauto.
+  split; auto.
+  SCase "wf_ECs_tail".
+    eapply wf_ECStack_head_tail_br; eauto.
+Qed.
+
+Lemma FBOP__wf_GVs_in_ECs : forall (v : value) (v0 : value) (id1 : id) 
+  (fbop0 : fbop) gvs3 TD fbop0 fp lc gl hd tl Mem0 td pinfo maxb 
+  (Hneq: PI_f pinfo = Opsem.CurFunction hd -> id1 <> PI_id pinfo)
+  (H11 : FBOP TD lc gl fbop0 fp v v0 = ret gvs3),
+  wf_GVs_in_ECs maxb pinfo td Mem0 hd tl id1 gvs3.
+Proof.
+  intros. 
+  unfold wf_GVs_in_ECs. destruct hd; simpl in *.
+  split.   
+    destruct (fdef_dec (PI_f pinfo) CurFunction); subst; auto.
+    intros.
+    assert (PI_f pinfo = PI_f pinfo) as EQ. auto.
+    apply Hneq in EQ. clear Hneq.
+    split; intros; subst; try congruence.
+      eapply FBOP_preserves_no_alias; eauto.
+  split.
+    intros. eapply FBOP_preserves_no_alias; eauto.
+    intros. subst. apply FBOP_preserves_no_embedded_ptrs in H11; auto.
+      apply no_embedded_ptrs__valid_ptrs; auto.
+Qed.
+
+Lemma insertGenericValue__wf_GVs_in_ECs : forall (v v': value) (id1 : id)
+  gvs2 TD gl EC Mem pinfo maxb t t'
+  (Hwflc: wf_lc Mem (@Opsem.Locals DGVs EC)) 
+  (Hwfgl: wf_globals maxb gl) (HwfM: maxb < Mem.nextblock Mem)
+  (Hwfv: Opsem.CurFunction EC = (PI_f pinfo) -> wf_use_at_head pinfo v) 
+  (Hwfv': Opsem.CurFunction EC = (PI_f pinfo) -> wf_use_at_head pinfo v') 
+  gvs gvs'
+  (Hneq: PI_f pinfo = Opsem.CurFunction EC -> id1 <> PI_id pinfo)
+  (H : Opsem.getOperandValue TD v (Opsem.Locals EC) gl = ret gvs) 
+  (H' : Opsem.getOperandValue TD v' (Opsem.Locals EC) gl = ret gvs') idxs
+  (H11 : ret gvs2 = Opsem.insertGenericValue TD t gvs idxs t' gvs') tl
+  (Hwfstk: 
+    wf_ECStack_head_tail maxb pinfo TD Mem (Opsem.Locals EC) tl),
+  wf_GVs_in_ECs maxb pinfo TD Mem EC tl id1 gvs2.
+Proof.
+  intros. 
+  unfold wf_GVs_in_ECs. destruct EC.
+  split.
+    destruct (fdef_dec (PI_f pinfo) CurFunction); subst; auto.
+    intros.
+    assert (PI_f pinfo = PI_f pinfo) as EQ. auto.
+    apply Hneq in EQ. clear Hneq.
+    split; intros; subst; try congruence.
+      eapply operand__no_alias_with__head with (als:=Allocas) (mptr0:=gvs)
+        (M:=Mem) in H; eauto.
+      eapply operand__no_alias_with__head with (als:=Allocas) (mptr0:=gvs')
+        (M:=Mem) in H'; eauto.
+      eapply insertGenericValue_preserves_no_alias in H11; eauto.
+  split.
+    intros.
+    eapply operand__no_alias_with__tail' in H; eauto.
+    eapply operand__no_alias_with__tail' in H'; eauto.
+    eapply insertGenericValue_preserves_no_alias in H11; eauto.
+
+    eapply insertGenericValue_preserves_valid_ptrs in H11; eauto.
+    eapply operand__lt_nextblock in H; eauto.
+    eapply operand__lt_nextblock in H'; eauto.
+Qed.
+
+Lemma extractGenericValue__wf_GVs_in_ECs : forall (v : value) (id1 : id)
+  gvs2 TD gl EC Mem pinfo maxb t 
+  (Hwflc: wf_lc Mem (@Opsem.Locals DGVs EC)) 
+  (Hwfgl: wf_globals maxb gl) (HwfM: maxb < Mem.nextblock Mem)
+  (Hwfv: Opsem.CurFunction EC = (PI_f pinfo) ->
+         wf_use_at_head pinfo v) gvs1
+  (Hneq: PI_f pinfo = Opsem.CurFunction EC -> id1 <> PI_id pinfo)
+  (H : Opsem.getOperandValue TD v (Opsem.Locals EC) gl = ret gvs1) idxs
+  (H11 : ret gvs2 = Opsem.extractGenericValue TD t gvs1 idxs) tl
+  (Hwfstk: 
+    wf_ECStack_head_tail maxb pinfo TD Mem (Opsem.Locals EC) tl),
+  wf_GVs_in_ECs maxb pinfo TD Mem EC tl id1 gvs2.
+Proof.
+  intros. 
+  unfold wf_GVs_in_ECs. destruct EC.
+  split.
+    destruct (fdef_dec (PI_f pinfo) CurFunction); subst; auto.
+    intros.
+    assert (PI_f pinfo = PI_f pinfo) as EQ. auto.
+    apply Hneq in EQ. clear Hneq.
+    split; intros; subst; try congruence.
+      eapply operand__no_alias_with__head with (als:=Allocas) (mptr0:=gvs1)
+        (M:=Mem) in H; eauto.
+        eapply extractGenericValue_preserves_no_alias in H11; eauto.
+  split.
+    intros.
+    eapply operand__no_alias_with__tail' in H; eauto.
+    eapply extractGenericValue_preserves_no_alias in H11; eauto.
+
+    eapply extractGenericValue_preserves_valid_ptrs in H11; eauto.
+    eapply operand__lt_nextblock in H; eauto.
+Qed.
+
+Lemma EXT__wf_GVs_in_ECs : forall (id1 : id) gvs2 TD gl EC Mem pinfo maxb
+  (Hwflc: wf_lc Mem (@Opsem.Locals DGVs EC)) v1
+  (Hwfgl: wf_globals maxb gl) (HwfM: maxb < Mem.nextblock Mem)
+  (Hwfv: Opsem.CurFunction EC = (PI_f pinfo) ->
+         wf_use_at_head pinfo v1) eop0 t1 t2 
+  (Hneq: PI_f pinfo = Opsem.CurFunction EC -> id1 <> PI_id pinfo)
+  (H11 : Opsem.EXT TD (Opsem.Locals EC) gl eop0 t1 v1 t2 = ret gvs2) tl
+  (Hwfstk: 
+    wf_ECStack_head_tail maxb pinfo TD Mem (Opsem.Locals EC) tl),
+  wf_GVs_in_ECs maxb pinfo TD Mem EC tl id1 gvs2.
+Proof.
+  intros. 
+  unfold wf_GVs_in_ECs. destruct EC.
+  apply OpsemProps.EXT_inversion in H11.
+  destruct H11 as [gv1 [J1 J2]].
+  unfold lift_op1 in J2. simpl in J2. unfold MDGVs.lift_op1 in J2.
+  split.
+    destruct (fdef_dec (PI_f pinfo) CurFunction); subst; auto.
+    intros.
+    assert (PI_f pinfo = PI_f pinfo) as EQ. auto.
+    apply Hneq in EQ. clear Hneq.
+    split; intros; subst; try congruence.
+      eapply operand__no_alias_with__head with (als:=Allocas) (mptr0:=gv1)
+        (M:=Mem) in J1; eauto.
+        eapply mext_preserves_no_alias in J2; eauto.
+  split.
+    intros.
+    eapply operand__no_alias_with__tail' in J1; eauto.
+    eapply mext_preserves_no_alias in J2; eauto.
+
+    eapply mext_preserves_valid_ptrs in J2; eauto.
+Qed.
+
+Lemma TRUNC__wf_GVs_in_ECs : forall (id1 : id) gvs2 TD gl EC Mem pinfo maxb
+  (Hwflc: wf_lc Mem (@Opsem.Locals DGVs EC)) v1
+  (Hwfgl: wf_globals maxb gl) (HwfM: maxb < Mem.nextblock Mem)
+  (Hwfv: Opsem.CurFunction EC = (PI_f pinfo) ->
+         wf_use_at_head pinfo v1) top0 t1 t2 
+  (Hneq: PI_f pinfo = Opsem.CurFunction EC -> id1 <> PI_id pinfo)
+  (H11 : Opsem.TRUNC TD (Opsem.Locals EC) gl top0 t1 v1 t2 = ret gvs2) tl
+  (Hwfstk: 
+    wf_ECStack_head_tail maxb pinfo TD Mem (Opsem.Locals EC) tl),
+  wf_GVs_in_ECs maxb pinfo TD Mem EC tl id1 gvs2.
+Proof.
+  intros. 
+  unfold wf_GVs_in_ECs. destruct EC.
+  apply OpsemProps.TRUNC_inversion in H11.
+  destruct H11 as [gv1 [J1 J2]].
+  unfold lift_op1 in J2. simpl in J2. unfold MDGVs.lift_op1 in J2.
+  split.
+    destruct (fdef_dec (PI_f pinfo) CurFunction); subst; auto.
+    intros.
+    assert (PI_f pinfo = PI_f pinfo) as EQ. auto.
+    apply Hneq in EQ. clear Hneq.
+    split; intros; subst; try congruence.
+      eapply operand__no_alias_with__head with (als:=Allocas) (mptr0:=gv1)
+        (M:=Mem) in J1; eauto.
+        eapply mtrunc_preserves_no_alias in J2; eauto.
+  split.
+    intros.
+    eapply operand__no_alias_with__tail' in J1; eauto.
+    eapply mtrunc_preserves_no_alias in J2; eauto.
+
+    eapply mtrunc_preserves_valid_ptrs in J2; eauto.
+Qed.
+
+Lemma ICMP__wf_GVs_in_ECs : forall (id1 : id) gvs2 TD gl EC Mem pinfo maxb
+  (Hwflc: wf_lc Mem (@Opsem.Locals DGVs EC)) v1 v2
+  (Hwfgl: wf_globals maxb gl) (HwfM: maxb < Mem.nextblock Mem)
+  (Hwfv1: Opsem.CurFunction EC = (PI_f pinfo) -> wf_use_at_head pinfo v1)
+  (Hwfv2: Opsem.CurFunction EC = (PI_f pinfo) -> wf_use_at_head pinfo v2)
+  cond0 t
+  (Hneq: PI_f pinfo = Opsem.CurFunction EC -> id1 <> PI_id pinfo)
+  (H11 : Opsem.ICMP TD (Opsem.Locals EC) gl cond0 t v1 v2 = ret gvs2) tl
+  (Hwfstk: 
+    wf_ECStack_head_tail maxb pinfo TD Mem (Opsem.Locals EC) tl),
+  wf_GVs_in_ECs maxb pinfo TD Mem EC tl id1 gvs2.
+Proof.
+  intros. 
+  unfold wf_GVs_in_ECs. destruct EC.
+  apply OpsemProps.ICMP_inversion in H11.
+  destruct H11 as [gv1 [gv2 [J1 [J2 J3]]]].
+  Local Transparent lift_op2.
+  unfold lift_op2 in J3. simpl in J3. unfold MDGVs.lift_op2 in J3.
+  split.
+    destruct (fdef_dec (PI_f pinfo) CurFunction); subst; auto.
+    intros.
+    assert (PI_f pinfo = PI_f pinfo) as EQ. auto.
+    apply Hneq in EQ. clear Hneq.
+    split; intros; subst; try congruence.
+      eapply operand__no_alias_with__head with (als:=Allocas) (mptr0:=gv1)
+        (M:=Mem) in J1; eauto.
+      eapply operand__no_alias_with__head with (als:=Allocas) (mptr0:=gv2)
+        (M:=Mem) in J2; eauto.
+      eapply micmp_preserves_no_alias in J3; eauto.
+  split.
+    intros.
+    eapply operand__no_alias_with__tail' in J1; eauto.
+    eapply operand__no_alias_with__tail' in J2; eauto.
+    eapply micmp_preserves_no_alias in J3; eauto.
+
+    eapply micmp_preserves_valid_ptrs in J3; eauto.
+Qed.
+
+
+Lemma FCMP__wf_GVs_in_ECs : forall (id1 : id) gvs2 TD gl EC Mem pinfo maxb
+  (Hwflc: wf_lc Mem (@Opsem.Locals DGVs EC)) v1 v2
+  (Hwfgl: wf_globals maxb gl) (HwfM: maxb < Mem.nextblock Mem)
+  (Hwfv1: Opsem.CurFunction EC = (PI_f pinfo) -> wf_use_at_head pinfo v1)
+  (Hwfv2: Opsem.CurFunction EC = (PI_f pinfo) -> wf_use_at_head pinfo v2)
+  fcond0 fp
+  (Hneq: PI_f pinfo = Opsem.CurFunction EC -> id1 <> PI_id pinfo)
+  (H11 : Opsem.FCMP TD (Opsem.Locals EC) gl fcond0 fp v1 v2 = ret gvs2) tl
+  (Hwfstk: 
+    wf_ECStack_head_tail maxb pinfo TD Mem (Opsem.Locals EC) tl),
+  wf_GVs_in_ECs maxb pinfo TD Mem EC tl id1 gvs2.
+Proof.
+  intros. 
+  unfold wf_GVs_in_ECs. destruct EC.
+  apply OpsemProps.FCMP_inversion in H11.
+  destruct H11 as [gv1 [gv2 [J1 [J2 J3]]]].
+  Local Transparent lift_op2.
+  unfold lift_op2 in J3. simpl in J3. unfold MDGVs.lift_op2 in J3.
+  split.
+    destruct (fdef_dec (PI_f pinfo) CurFunction); subst; auto.
+    intros.
+    assert (PI_f pinfo = PI_f pinfo) as EQ. auto.
+    apply Hneq in EQ. clear Hneq.
+    split; intros; subst; try congruence.
+      eapply operand__no_alias_with__head with (als:=Allocas) (mptr0:=gv1)
+        (M:=Mem) in J1; eauto.
+      eapply operand__no_alias_with__head with (als:=Allocas) (mptr0:=gv2)
+        (M:=Mem) in J2; eauto.
+      eapply mfcmp_preserves_no_alias in J3; eauto.
+  split.
+    intros.
+    eapply operand__no_alias_with__tail' in J1; eauto.
+    eapply operand__no_alias_with__tail' in J2; eauto.
+    eapply mfcmp_preserves_no_alias in J3; eauto.
+
+    eapply mfcmp_preserves_valid_ptrs in J3; eauto.
+Qed.
+
+Lemma getOperandValue__wf_GVs_in_ECs : forall (v : value) (id1 : id)
+  TD gl EC Mem pinfo maxb  
+  (Hwflc: wf_lc Mem (@Opsem.Locals DGVs EC)) 
+  (Hwfgl: wf_globals maxb gl) (HwfM: maxb < Mem.nextblock Mem)
+  (Hwfv: Opsem.CurFunction EC = (PI_f pinfo) ->
+         wf_use_at_head pinfo v) gvs
+  (Hneq: PI_f pinfo = Opsem.CurFunction EC -> id1 <> PI_id pinfo)
+  (H : Opsem.getOperandValue TD v (Opsem.Locals EC) gl = ret gvs) tl
+  (Hwfstk: 
+    wf_ECStack_head_tail maxb pinfo TD Mem (Opsem.Locals EC) tl),
+  wf_GVs_in_ECs maxb pinfo TD Mem EC tl id1 gvs.
+Proof.
+  intros. 
+  unfold wf_GVs_in_ECs. destruct EC.
+  split.
+    destruct (fdef_dec (PI_f pinfo) CurFunction); subst; auto.
+    intros.
+    assert (PI_f pinfo = PI_f pinfo) as EQ. auto.
+    apply Hneq in EQ. clear Hneq.
+    split; intros; subst; try congruence.
+      eapply operand__no_alias_with__head with (mptr0:=gvs) (M:=Mem) in H1; 
+        eauto.
+  split.
+    intros.
+    eapply operand__no_alias_with__tail' in H; eauto.
+    eapply operand__lt_nextblock in H; eauto.
+Qed.
+
+Ltac preservation_tac0:=
+  match goal with
+  | HwfPI : WF_PhiInfo _ ,
+    HFinPs1: InProductsB _ _ = _,
+    HBinF1: blockInFdefB _ _ = _,
+    HmInS: moduleInSystemB _ _ = _,
+    HwfSystem: wf_system _ _ |- _ =>
+    clear - HBinF1 HFinPs1 HmInS HwfPI HwfSystem;
+    simpl; intros; subst;
+    eapply wf_system__uniqFdef in HFinPs1; eauto; 
+    intro J; subst;
+    apply PhiInfo_must_be_promotable_alloca in HBinF1;
+              try solve [auto | inv HBinF1 | intros; congruence]
+  end.
+
+Ltac preservation_tac1:=
+match goal with
+| Hinv : OpsemPP.wf_State _ _,
+  HwfS1 : wf_State _ _ _ _,
+  HwfPI : WF_PhiInfo _ |- _ =>
+  simpl_ctx Hinv HwfS1;
+  preservation_tac0
+end.
+
+Ltac preservation_tac2:=
+  match goal with
+  | HwfPI : WF_PhiInfo _,
+    HFinPs1: InProductsB _ _ = _,
+    HBinF1: blockInFdefB _ _ = _,
+    HmInS: moduleInSystemB _ _ = _,
+    HwfSystem: wf_system _ _ |- _ =>
+    clear - HBinF1 HFinPs1 HmInS HwfPI HwfSystem;
+    simpl; intros; subst;
+    eapply wf_system__uniqFdef in HFinPs1; eauto;
+    eapply IngetCmdsIDs__lookupCmdViaIDFromFdef in HBinF1; 
+      eauto using in_middle;
+    eapply WF_PhiInfo_spec4 in HBinF1; eauto; simpl; auto
+  end.
+
+Ltac preservation_tac3 :=
+  match goal with
+  | Hinv : OpsemPP.wf_State _ _,
+    HwfS1 : wf_State _ _ _ _,
+    HwfPI : WF_PhiInfo _ |- _ =>
+    simpl_ctx Hinv HwfS1;
+    preservation_tac2
+  end.
+
+
+Ltac simpl_ctx' Hinv HwfS1 :=
+  destruct Hinv as 
+    [_ [HwfSystem [HmInS [Hnonempty [
+     [Hreach1 [HBinF1 [HFinPs1 [_ [_ [l1 [ps1 [cs1' Heq1]]]]]]]] 
+     [HwfEC0 HwfCall]
+    ]]]]]; subst;
+  fold (@OpsemPP.wf_ECStack DGVs) in HwfEC0;
+  destruct HwfS1 as [[[_ Hwflc] [HwfECs Hwfht]] [Hnonup1 [_ HwfM]]].
+
+Lemma preservation : forall maxb pinfo cfg S1 S2 tr
+  (Hinv: OpsemPP.wf_State cfg S1)
+  (Hwfg: wf_globals maxb (OpsemAux.Globals cfg)) (Hinbd: 0 <= maxb)
+  (HwfPI: WF_PhiInfo pinfo) (HsInsn: Opsem.sInsn cfg S1 S2 tr)
+  (HwfS1: wf_State maxb pinfo cfg S1), wf_State maxb pinfo cfg S2.
+Proof.
+  intros.
+  (sInsn_cases (induction HsInsn) Case); destruct TD as [los nts]; simpl HwfS1.
+
+Case "sReturn". eapply preservation_return; eauto. 
+Case "sReturnVoid". eapply preservation_return_void; eauto. 
+Case "sBranch". eapply preservation_branch in Hinv; eauto.
+Case "sBranch_uncond". eapply preservation_branch_uncond in Hinv; eauto.
+
+Case "sBop".
+  eapply preservation_pure_cmd_updated_case in HwfS1; try solve [simpl; eauto]; 
+    eauto.
+    eapply BOP__wf_GVs_in_ECs; eauto.
+      preservation_tac1.
+
+Case "sFBop".
+  eapply preservation_pure_cmd_updated_case in HwfS1; try solve [simpl; eauto]; 
+    eauto.
+    eapply FBOP__wf_GVs_in_ECs; eauto.
+      preservation_tac1.
+
+Case "sExtractValue".
+  eapply preservation_pure_cmd_updated_case in HwfS1; try solve [simpl; eauto]; 
+    eauto.
+    simpl_ctx' Hinv HwfS1.
+    eapply extractGenericValue__wf_GVs_in_ECs; simpl;
+      try solve [eauto | preservation_tac2 | preservation_tac0].
+
+Case "sInsertValue". 
+  eapply preservation_pure_cmd_updated_case in HwfS1; try solve [simpl; eauto]; 
+    eauto.
+    simpl_ctx' Hinv HwfS1.
+    eapply insertGenericValue__wf_GVs_in_ECs with (v:=v) (gvs:=gvs) (v':=v')
+      (gvs':=gvs'); try solve [eauto | preservation_tac2 | preservation_tac0].
+
+Case "sMalloc". 
+  assert (PI_f pinfo = F -> id0 <> PI_id pinfo) as Hneq. 
+    preservation_tac1.
+  simpl_ctx Hinv HwfS1.
+  split.
+    split.
+      eapply impure_cmd_updated_preserves_wf_EC; eauto.
+        intros. subst.
+        apply wf_EC__wf_lc in HwfEC.
+        eapply malloc_preserves_wf_defs_at_head; eauto.
+        eapply malloc_preserves_wf_lc; eauto.
+    split.
+      eapply malloc_preserves_wf_ECStack_in_tail in H2; eauto.
+      eapply malloc_preserves_wf_ECStack_head_tail in H2; eauto.
+  split.
+    destruct HwfM1.
+    eapply malloc_preserves_wf_als in H2; eauto.
+      simpl_env in H2.
+      apply wf_als_split in H2. destruct H2; auto.
+    eapply malloc_preserves_wf_Mem in H2; eauto.
+
+Case "sFree". 
+  simpl_ctx Hinv HwfS1.
+  split.
+    split.
+      eapply impure_cmd_non_updated_preserves_wf_EC with (M:=Mem); eauto.
+        intros. subst.
+        eapply free_preserves_wf_defs_at_head; eauto.
+          preservation_tac2.
+        eapply free_preserves_wf_lc; eauto.
+    split.
+      eapply free_preserves_wf_ECStack_in_tail in H1; eauto.
+      eapply free_preserves_wf_ECStack_head_tail in H1; eauto.
+  split.
+    eapply free_preserves_wf_als in H1; eauto.
+    eapply free_preserves_wf_Mem in H1; eauto.
+
+Case "sAlloca". 
+  simpl_ctx Hinv HwfS1.
+  split.
+    split.
+      eapply impure_cmd_updated_preserves_wf_EC; eauto.
+        intros. subst.
+        apply wf_EC__wf_lc in HwfEC.
+
+        eapply wf_system__wf_fdef in HwfSystem; eauto.
+        eapply alloca_preserves_wf_defs_at_head; eauto.
+         
+        eapply malloc_preserves_wf_lc; eauto.
+    split.       
+      eapply malloc_preserves_wf_ECStack_in_tail in H2; eauto.
+      eapply malloc_preserves_wf_ECStack_head_tail in H2; eauto.
+  split.
+    destruct HwfM1.
+    eapply malloc_preserves_wf_als in H2; eauto.
+    eapply malloc_preserves_wf_Mem in H2; eauto.
+
+Case "sLoad". 
+  eapply preservation_pure_cmd_updated_case in HwfS1; try solve [simpl; eauto]; 
+    eauto.
+    assert (PI_f pinfo = F -> id0 <> PI_id pinfo) as Hneq. 
+      preservation_tac1.
+    destruct HwfS1 as [[[_ Hwflc] [_ Hwfstk]] [_ HwfM]]. 
+    eapply mload__wf_GVs_in_ECs; eauto using wf_EC__wf_lc.
+
+Case "sStore". 
+  simpl_ctx Hinv HwfS1.
+  assert (wf_lc Mem lc) as Hwflc.
+    apply wf_EC__wf_lc in HwfEC; auto.
+  split.
+    split.
+      eapply impure_cmd_non_updated_preserves_wf_EC with (M:=Mem); eauto.
+        intros. subst.
+        eapply mstore_preserves_wf_defs_at_head with (gvs1:=gvs1) in H3; eauto.
+          preservation_tac2.
+        eapply mstore_preserves_wf_lc; eauto.
+    split.
+      eapply mstore_preserves_wf_ECStack_in_tail with (gvs1:=gvs1) in H3; eauto.
+      eapply mstore_preserves_wf_ECStack_head_tail' with (gvs1:=gvs1) in H3; 
+        eauto.
+  split.
+    eapply mstore_preserves_wf_als in H3; eauto.
+    eapply mstore_preserves_wf_Mem with (gvs1:=gvs1) in H3; eauto.
+
+Case "sGEP". 
+  eapply preservation_pure_cmd_updated_case in HwfS1; try solve [simpl; eauto]; 
+    eauto.
+    simpl_ctx' Hinv HwfS1.
+    eapply GEP__wf_GVs_in_ECs; try solve 
+      [eauto using wf_EC__wf_lc | preservation_tac2 | preservation_tac0].
+
+Case "sTrunc".
+  eapply preservation_pure_cmd_updated_case in HwfS1; try solve [simpl; eauto]; 
+    eauto.
+    simpl_ctx' Hinv HwfS1.
+    eapply TRUNC__wf_GVs_in_ECs; 
+      try solve [eauto | preservation_tac2 | preservation_tac0].
+
+Case "sExt".
+  eapply preservation_pure_cmd_updated_case in HwfS1; try solve [simpl; eauto]; 
+    eauto.
+    simpl_ctx' Hinv HwfS1.
+    eapply EXT__wf_GVs_in_ECs;
+      try solve [eauto | preservation_tac2 | preservation_tac0].
+
+Case "sCast". 
+  eapply preservation_pure_cmd_updated_case in HwfS1; try solve [simpl; eauto]; 
+    eauto.
+    simpl_ctx' Hinv HwfS1.
+    eapply CAST__wf_GVs_in_ECs;
+      try solve [eauto | preservation_tac2 | preservation_tac0].
+
+Case "sIcmp". 
+  eapply preservation_pure_cmd_updated_case in HwfS1; try solve [simpl; eauto]; 
+    eauto.
+    simpl_ctx' Hinv HwfS1.
+    eapply ICMP__wf_GVs_in_ECs with (v1:=v1)(v2:=v2);
+      try solve [eauto | preservation_tac2 | preservation_tac0].
+
+Case "sFcmp". 
+  eapply preservation_pure_cmd_updated_case in HwfS1; try solve [simpl; eauto]; 
+    eauto.
+    simpl_ctx' Hinv HwfS1.
+    eapply FCMP__wf_GVs_in_ECs with (v1:=v1)(v2:=v2);
+      try solve [eauto | preservation_tac2 | preservation_tac0].
+
+Case "sSelect". 
+  destruct (isGVZero (los, nts) c);
+    eapply preservation_pure_cmd_updated_case in HwfS1; try solve [simpl; eauto]; 
+      try solve [eauto | 
+                 simpl_ctx' Hinv HwfS1;
+                 match goal with
+                 | H1: Opsem.getOperandValue _ ?v1 _ _ = ret ?gvs1 |- 
+                       wf_GVs_in_ECs _ _ _ _ _ _ _ ?gvs1 => 
+                   eapply getOperandValue__wf_GVs_in_ECs with (v:=v1); 
+                     try solve [eauto | preservation_tac2 | preservation_tac0]
+                 end].
+
+Case "sCall". eapply preservation_Call; eauto.
 
 Case "sExCall". 
   destruct HwfS1 as [[HwfEC [HwfECs Hwfht]] [Hnonup1 HwfM1]].
@@ -2493,6 +3692,8 @@ Case "sExCall".
       eapply callExternalFunction_preserves_wf_als; eauto.
       eapply callExternalFunction_preserves_wf_Mem; eauto.
 Qed.
+
+Opaque lift_op1. 
 
 End Promotability.
 
